Syntactic translation

simple-frontend/FrontEndTranslation.thy
@@ -20,13 +20,13 @@ lemma semantify_addr_equiv:
   using semantify_addr_def by auto
 
 lemma convert_proof_assign:
-  assumes "ConcreteSemantics.SL_proof \<Delta> A (abs_stmt.LocalAssign x (semantify_exp e)) B"
-  shows "\<Delta> \<turnstile>CSL [A] Cassign x e [B]"
+  assumes "ConcreteSemantics.SL_proof tcfe A (abs_stmt.LocalAssign x (semantify_exp e)) B"
+  shows "tcfe \<turnstile>CSL [A] Cassign x e [B]"
 proof -
   have "B = ConcreteSemantics.post_substitute_var_assert x (semantify_exp e) A"
     using ConcreteSemantics.SL_proof_LocalAssign_elim assms
     by fast
-  moreover have "\<Delta> \<turnstile>CSL [A] Cassign x e [ConcreteSemantics.post_substitute_var_assert x (semantify_exp e) A]"
+  moreover have "tcfe \<turnstile>CSL [A] Cassign x e [ConcreteSemantics.post_substitute_var_assert x (semantify_exp e) A]"
   proof (rule RuleCons)
     show "A \<subseteq> sub_pre x e (ConcreteSemantics.post_substitute_var_assert x (semantify_exp e) A)"
       unfolding sub_pre_def ConcreteSemantics.post_substitute_var_assert_def ConcreteSemantics.substitute_var_state_def TypedEqui.assign_var_state_def
@@ -39,159 +39,183 @@ proof -
       ultimately show "\<exists>s \<tau> \<omega>. (a, aa, b) = (Ag s, \<tau>, \<omega>) \<and> (Ag (s(x \<mapsto> VInt (edenot e s))), \<tau>, \<omega>) \<in> (\<lambda>\<omega>. set_store \<omega> ((get_store \<omega>)(x := semantify_exp e \<omega>))) ` A"
         by blast
     qed
-    show "\<Delta> \<turnstile>CSL [sub_pre x e (ConcreteSemantics.post_substitute_var_assert x (semantify_exp e) A)] Cassign x e [ConcreteSemantics.post_substitute_var_assert x (semantify_exp e) A]"
+    show "tcfe \<turnstile>CSL [sub_pre x e (ConcreteSemantics.post_substitute_var_assert x (semantify_exp e) A)] Cassign x e [ConcreteSemantics.post_substitute_var_assert x (semantify_exp e) A]"
       by (simp add: RuleAssign)
   qed (simp)
   ultimately show ?thesis by auto
 qed
 
 lemma convert_proof_skip:
-  assumes "ConcreteSemantics.SL_proof \<Delta> A Skip B"
-  shows "\<Delta> \<turnstile>CSL [A] Cskip [B]"
+  assumes "ConcreteSemantics.SL_proof tcfe A Skip B"
+  shows "tcfe \<turnstile>CSL [A] Cskip [B]"
   using RuleSkip assms by blast
 
 lemma conjunct_with_true_entails:
-  assumes "TypedEqui.typed_assertion \<Delta> P"
-  shows "P \<subseteq> atrue \<Delta> \<otimes> P"
+  assumes "TypedEqui.typed_assertion tcfe P"
+  shows "P \<subseteq> atrue tcfe \<otimes> P"
 proof
   fix \<omega> assume "\<omega> \<in> P"
   then have "Some \<omega> = |\<omega>| \<oplus> \<omega>"
     by (simp add: commutative core_is_smaller)
-  moreover have "|\<omega>| \<in> atrue \<Delta>"
+  moreover have "|\<omega>| \<in> atrue tcfe"
     by (metis CollectI TypedEqui.typed_core TypedEqui.typed_state_axioms \<open>\<omega> \<in> P\<close> assms TypedEqui.atrue_def typed_state.typed_assertionE)
-  ultimately show "\<omega> \<in> atrue \<Delta> \<otimes> P"
+  ultimately show "\<omega> \<in> atrue tcfe \<otimes> P"
     using \<open>\<omega> \<in> P\<close> x_elem_set_product by blast
 qed
 
 (*
 definition make_semantic_assertion :: "('a, 'a virtual_state) interp \<Rightarrow> (field_name \<rightharpoonup> vtyp) \<Rightarrow> (pure_exp, pure_exp atomic_assert) assert \<Rightarrow> 'a equi_state set" where
-  "make_semantic_assertion \<Delta> F A = well_typedly \<Delta> F (\<langle>\<Delta>, F\<rangle> \<Turnstile> \<langle>A\<rangle>)"
+  "make_semantic_assertion tcfe F A = well_typedly tcfe F (\<langle>type_ctxt_front_end, F\<rangle> \<Turnstile> \<langle>A\<rangle>)"
 *)
 
 
+abbreviation tcfe :: "(int val, char list \<Rightarrow> int val set option) abs_type_context" where
+  "tcfe \<equiv> type_ctxt_front_end"
+
+
+
 fun wf_stmt where
-  "wf_stmt \<Gamma> F \<Delta> (Cseq C1 C2) \<longleftrightarrow> wf_stmt \<Gamma> F \<Delta> C1 \<and> wf_stmt \<Gamma> F \<Delta> C2"
-| "wf_stmt \<Gamma> F \<Delta> (Calloc r e) \<longleftrightarrow> r \<notin> fvE e"
+  "wf_stmt \<Gamma> F (Cseq C1 C2) \<longleftrightarrow> wf_stmt \<Gamma> F C1 \<and> wf_stmt \<Gamma> F C2"
+| "wf_stmt \<Gamma> F (Calloc r e) \<longleftrightarrow> r \<notin> fvE e"
 
-| "wf_stmt \<Gamma> F \<Delta> ({P1} C1 {Q1} || {P2} C2 {Q2}) \<longleftrightarrow>
-  disjoint (fvC C1 \<union> fvA \<Delta> ((make_semantic_assertion \<Gamma> F Q1) \<otimes> atrue \<Delta>)) (wrC C2) \<and> disjoint (fvC C2 \<union> fvA \<Delta> ((make_semantic_assertion \<Gamma> F Q2) \<otimes> atrue \<Delta>)) (wrC C1) \<and>
-  TypedEqui.self_framing_typed \<Delta> (make_semantic_assertion \<Gamma> F P1) \<and> TypedEqui.typed_assertion \<Delta> (make_semantic_assertion \<Gamma> F P1) \<and>
-  TypedEqui.self_framing_typed \<Delta> (make_semantic_assertion \<Gamma> F P2) \<and> TypedEqui.typed_assertion \<Delta> (make_semantic_assertion \<Gamma> F P2) \<and>
-  wf_stmt \<Gamma> F \<Delta> C1 \<and> wf_stmt \<Gamma> F \<Delta> C2"
+| "wf_stmt \<Gamma> F ({P1} C1 {Q1} || {P2} C2 {Q2}) \<longleftrightarrow>
+  disjoint (fvC C1 \<union> fvA tcfe ((make_semantic_assertion \<Gamma> type_ctxt_front_end_syntactic Q1) \<otimes> atrue tcfe)) (wrC C2) \<and> disjoint (fvC C2 \<union> fvA tcfe ((make_semantic_assertion \<Gamma> type_ctxt_front_end_syntactic Q2) \<otimes> atrue tcfe)) (wrC C1) \<and>
+  TypedEqui.self_framing_typed tcfe (make_semantic_assertion \<Gamma> type_ctxt_front_end_syntactic P1) \<and> TypedEqui.typed_assertion tcfe (make_semantic_assertion \<Gamma> type_ctxt_front_end_syntactic P1) \<and>
+  TypedEqui.self_framing_typed tcfe (make_semantic_assertion \<Gamma> type_ctxt_front_end_syntactic P2) \<and> TypedEqui.typed_assertion tcfe (make_semantic_assertion \<Gamma> type_ctxt_front_end_syntactic P2) \<and>
+  wf_stmt \<Gamma> F C1 \<and> wf_stmt \<Gamma> F C2"
 
-| "wf_stmt \<Gamma> F \<Delta> (Cif b C1 C2) \<longleftrightarrow> wf_stmt \<Gamma> F \<Delta> C1 \<and> wf_stmt \<Gamma> F \<Delta> C2"
+| "wf_stmt \<Gamma> F (Cif b C1 C2) \<longleftrightarrow> wf_stmt \<Gamma> F C1 \<and> wf_stmt \<Gamma> F C2"
 
-| "wf_stmt \<Gamma> F \<Delta> (Cwhile b I C) \<longleftrightarrow> TypedEqui.self_framing_typed \<Delta> (make_semantic_assertion \<Gamma> F I)
-                              \<and> TypedEqui.typed_assertion \<Delta> (make_semantic_assertion \<Gamma> F I) \<and> wf_stmt \<Gamma> F \<Delta> C"
+| "wf_stmt \<Gamma> F (Cwhile b I C) \<longleftrightarrow> TypedEqui.self_framing_typed tcfe (make_semantic_assertion \<Gamma> type_ctxt_front_end_syntactic I)
+                              \<and> TypedEqui.typed_assertion tcfe (make_semantic_assertion \<Gamma> type_ctxt_front_end_syntactic I) \<and> wf_stmt \<Gamma> F C"
 
-| "wf_stmt \<Gamma> F \<Delta> _ \<longleftrightarrow> True"
+| "wf_stmt \<Gamma> F _ \<longleftrightarrow> True"
 
 lemma atrue_self_framing_and_typed[simp]:
-  "TypedEqui.typed_assertion \<Delta> (atrue \<Delta>)"
-  "TypedEqui.self_framing_typed \<Delta> (atrue \<Delta>)"
+  "TypedEqui.typed_assertion tcfe (atrue tcfe)"
+  "TypedEqui.self_framing_typed tcfe (atrue tcfe)"
   using TypedEqui.typed_assertionI TypedEqui.atrue_def apply blast
   by (simp add: TypedEqui.self_framing_typedI TypedEqui.typed_state_then_stabilize_typed TypedEqui.atrue_def)
 
+abbreviation typed_stabilize where
+  "typed_stabilize \<equiv> TypedEqui.Stabilize_typed tcfe"
+
+lemma wf_context_type_context[simp]:
+  "TypedEqui.wf_context tcfe"
+  unfolding TypedEqui.wf_context_def
+proof -
+  have "dom (variables tcfe) \<subseteq> {x. x < undefined}"
+    by (metis CollectI abs_type_context.select_convs(1) domIff subsetI type_ctxt_front_end_def type_ctxt_store_def)
+  then show "finite (dom (variables tcfe))"
+    by (simp add: finite_subset)
+qed
+
+lemma typed_stabi_atrue[simp]:
+  "typed_stabilize (atrue tcfe) = atrue tcfe"
+  by (metis (no_types, opaque_lifting) ConcreteSemantics.stabilize_typed_elem TypedEqui.self_framing_Stabilize_typed TypedEqui.self_framing_typed_ext TypedEqui.typed_Stabilize_typed already_stable atrue_self_framing_and_typed(1) atrue_self_framing_and_typed(2))
+
 lemma convert_proof_alloc:
-  assumes "ConcreteSemantics.SL_proof \<Delta> P (Havoc r;; Inhale (full_ownership_with_val r e)) Q"
-      and "well_typed_cmd \<Delta> (Calloc r e)"
-      and "wf_stmt \<Gamma> F \<Delta> (Calloc r e)"
-      and "TypedEqui.wf_context \<Delta>"
-  shows "\<Delta> \<turnstile>CSL [P] Calloc r e [Q]"
+  assumes "ConcreteSemantics.SL_proof tcfe P (Havoc r;; Inhale (typed_stabilize (full_ownership_with_val r e))) Q"
+      and "well_typed_cmd tcfe (Calloc r e)"
+      and "wf_stmt \<Gamma> type_ctxt_front_end_syntactic (Calloc r e)"
+  shows "tcfe \<turnstile>CSL [P] Calloc r e [Q]"
 proof (rule RuleCons)
 
-  have asm0: "ConcreteSemantics.SL_proof \<Delta> P (Havoc r) (TypedEqui.exists_assert \<Delta> r P)
-  \<and> ConcreteSemantics.SL_proof \<Delta> (TypedEqui.exists_assert \<Delta> r P) (Inhale (full_ownership_with_val r e)) Q
-  \<and> TypedEqui.self_framing_typed \<Delta> P"
+  have asm0: "ConcreteSemantics.SL_proof tcfe P (Havoc r) (TypedEqui.exists_assert tcfe r P)
+  \<and> ConcreteSemantics.SL_proof tcfe (TypedEqui.exists_assert tcfe r P) (Inhale (typed_stabilize (full_ownership_with_val r e))) Q
+  \<and> TypedEqui.self_framing_typed tcfe P"
     by (metis ConcreteSemantics.SL_proof_Havoc_elim ConcreteSemantics.SL_proof_Seq_elim assms(1))
-  then have "Q = TypedEqui.exists_assert \<Delta> r P \<otimes> full_ownership_with_val r e"
+  then have "Q = TypedEqui.exists_assert tcfe r P \<otimes> typed_stabilize (full_ownership_with_val r e)"
     by blast
 
-  show "\<Delta> \<turnstile>CSL [atrue \<Delta> \<otimes> TypedEqui.exists_assert \<Delta> r P] Calloc r e [full_ownership_with_val r e \<otimes> TypedEqui.exists_assert \<Delta> r P]"
+  show "tcfe \<turnstile>CSL [atrue tcfe \<otimes> TypedEqui.exists_assert tcfe r P] Calloc r e [typed_stabilize (full_ownership_with_val r e) \<otimes> TypedEqui.exists_assert tcfe r P]"
   proof (rule RuleFrame)
     have "r \<notin> fvE e"
       using assms(3) by auto
-    then show "\<Delta> \<turnstile>CSL [atrue \<Delta>] Calloc r e [full_ownership_with_val r e]"
+    then have "tcfe \<turnstile>CSL [atrue tcfe] Calloc r e [full_ownership_with_val r e]"
       using RuleAlloc[of r e] by simp
-    show "disjoint (fvA \<Delta> (TypedEqui.exists_assert \<Delta> r P)) (wrC (Calloc r e))"
-      by (metis (no_types, lifting) ConcreteSemantics.SL_proof_Havoc_elim ConcreteSemantics.exists_assert_no_in_fv asm0 assms(4) disjoint_def disjoint_iff singletonD subset_Diff_insert wrC.simps(5))
-    show "TypedEqui.self_framing_typed \<Delta> (atrue \<Delta>)"
+    then show "tcfe \<turnstile>CSL [atrue tcfe] Calloc r e [typed_stabilize (full_ownership_with_val r e)]"
+      using RuleStabilizeTyped by fastforce
+
+    show "disjoint (fvA tcfe (TypedEqui.exists_assert tcfe r P)) (wrC (Calloc r e))"
+      by (metis (no_types, lifting) ConcreteSemantics.SL_proof_Havoc_elim ConcreteSemantics.exists_assert_no_in_fv asm0 disjoint_def disjoint_iff singletonD subset_Diff_insert wf_context_type_context wrC.simps(5))
+
+    show "TypedEqui.self_framing_typed tcfe (atrue tcfe)"
       using TypedEqui.self_framing_typed_def TypedEqui.atrue_def
       using TypedEqui.typed_state_then_stabilize_typed by blast
-    show "TypedEqui.self_framing_typed \<Delta> (TypedEqui.exists_assert \<Delta> r P)"
+    show "TypedEqui.self_framing_typed tcfe (TypedEqui.exists_assert tcfe r P)"
       using asm0 by fastforce
-    show "TypedEqui.typed_assertion \<Delta> (TypedEqui.exists_assert \<Delta> r P)"
+    show "TypedEqui.typed_assertion tcfe (TypedEqui.exists_assert tcfe r P)"
       using asm0 by fastforce
-    show "TypedEqui.typed_assertion \<Delta> (atrue \<Delta>)"
+    show "TypedEqui.typed_assertion tcfe (atrue tcfe)"
       using TypedEqui.typed_assertion_def TypedEqui.atrue_def by blast
   qed
 
-  moreover have "TypedEqui.typed_assertion \<Delta> P \<and> variables \<Delta> r \<noteq> None"
+  moreover have "TypedEqui.typed_assertion tcfe P \<and> variables tcfe r \<noteq> None"
   proof
-    show "TypedEqui.typed_assertion \<Delta> P"
+    show "TypedEqui.typed_assertion tcfe P"
       using asm0 by blast
-    show "variables \<Delta> r \<noteq> None"
-      using assms(2) by auto
+    show "variables tcfe r \<noteq> None"
+      by (metis assms(2) option.distinct(1) well_typed_cmd_aux.simps(6))
   qed
-  then have "entails P (TypedEqui.exists_assert \<Delta> r P)"
-    using ConcreteSemantics.SL_proof_Havoc_elim_entails[of \<Delta> P r "TypedEqui.exists_assert \<Delta> r P"]    
+  then have "entails P (TypedEqui.exists_assert tcfe r P)"
+    using ConcreteSemantics.SL_proof_Havoc_elim_entails[of tcfe P r "TypedEqui.exists_assert tcfe r P"]    
     using ConcreteSemantics.exists_assert_entails by blast
 
-  then show "P \<subseteq> atrue \<Delta> \<otimes> TypedEqui.exists_assert \<Delta> r P"
-    by (meson TypedEqui.typed_assertion_exists_assert \<open>TypedEqui.typed_assertion \<Delta> P \<and> variables \<Delta> r \<noteq> None\<close> conjunct_with_true_entails dual_order.trans entails_def)
-  show "full_ownership_with_val r e \<otimes> TypedEqui.exists_assert \<Delta> r P \<subseteq> Q"
-    by (simp add: \<open>Q = TypedEqui.exists_assert \<Delta> r P \<otimes> full_ownership_with_val r e\<close> add_set_commm)
+  then show "P \<subseteq> atrue tcfe \<otimes> TypedEqui.exists_assert tcfe r P"
+    by (meson TypedEqui.typed_assertion_exists_assert \<open>TypedEqui.typed_assertion tcfe P \<and> variables tcfe r \<noteq> None\<close> conjunct_with_true_entails dual_order.trans entails_def)
+  
+  show "typed_stabilize (full_ownership_with_val r e) \<otimes> TypedEqui.exists_assert tcfe r P \<subseteq> Q"
+    by (simp add: \<open>Q = TypedEqui.exists_assert tcfe r P \<otimes> typed_stabilize (full_ownership_with_val r e)\<close> add_set_commm)
 qed
 
 lemma helper_exhale_encoding:
-  assumes "ConcreteSemantics.SL_proof \<Delta> P (Exhale (Stabilize A)) Q"
-  shows "P \<subseteq> TypedEqui.Stabilize_typed \<Delta> A \<otimes> Q"
+  assumes "ConcreteSemantics.SL_proof tcfe P (Exhale (typed_stabilize A)) Q"
+  shows "P \<subseteq> typed_stabilize A \<otimes> Q"
   using assms(1)
 proof (rule ConcreteSemantics.SL_proof_Exhale_elim)
-  assume asm0: "entails P (Q \<otimes> Stabilize A)" "TypedEqui.self_framing_typed \<Delta> P"
-    "TypedEqui.typed_assertion \<Delta> P" "TypedEqui.self_framing_typed \<Delta> Q"
-    "TypedEqui.typed_assertion \<Delta> Q"
-  show "P \<subseteq> TypedEqui.Stabilize_typed \<Delta> A \<otimes> Q"
+  assume asm0: "entails P (Q \<otimes> typed_stabilize A)" "TypedEqui.self_framing_typed tcfe P"
+    "TypedEqui.typed_assertion tcfe P" "TypedEqui.self_framing_typed tcfe Q"
+    "TypedEqui.typed_assertion tcfe Q"
+  show "P \<subseteq> typed_stabilize A \<otimes> Q"
   proof
     fix \<omega> assume asm1: "\<omega> \<in> P"
-    then obtain q a where "q \<in> Q" "a \<in> Stabilize A" "Some \<omega> = q \<oplus> a"
+    then obtain q a where "q \<in> Q" "a \<in> typed_stabilize A" "Some \<omega> = q \<oplus> a"
       by (meson asm0(1) entails_def subsetD x_elem_set_product)
-    moreover have "TypedEqui.typed \<Delta> a"
+    moreover have "TypedEqui.typed tcfe a"
       using TypedEqui.typed_state_axioms asm0(3) asm1 calculation(3) greater_equiv typed_state.typed_assertionE typed_state.typed_smaller by blast
     then have "stabilize a \<in> A"
-      using calculation(2) by auto
-    thm TypedEqui.Stabilize_typed_def Stabilize_def
-
-    then show "\<omega> \<in> TypedEqui.Stabilize_typed \<Delta> A \<otimes> Q"
-      by (metis (no_types, lifting) ConcreteSemantics.stabilize_typed_elem \<open>TypedEqui.typed \<Delta> a\<close> calculation(1) calculation(3) commutative x_elem_set_product)
+      using ConcreteSemantics.stabilize_typed_elem calculation(2) by blast
+    then show "\<omega> \<in> TypedEqui.Stabilize_typed tcfe A \<otimes> Q"
+      by (metis (no_types, lifting) ConcreteSemantics.stabilize_typed_elem \<open>TypedEqui.typed tcfe a\<close> calculation(1) calculation(3) commutative x_elem_set_product)
   qed
 qed
 
 lemma convert_proof_free:
-  assumes "ConcreteSemantics.SL_proof \<Delta> P (Exhale (Stabilize (full_ownership r))) Q"
-  shows "\<Delta> \<turnstile>CSL [P] Cfree r [Q \<otimes> atrue \<Delta>]"
+  assumes "ConcreteSemantics.SL_proof tcfe P (Exhale (typed_stabilize (full_ownership r))) Q"
+  shows "tcfe \<turnstile>CSL [P] Cfree r [Q \<otimes> atrue tcfe]"
   using assms(1)
 proof (rule ConcreteSemantics.SL_proof_Exhale_elim)
-  assume asm0: "entails P (Q \<otimes> Stabilize (full_ownership r))" "TypedEqui.self_framing_typed \<Delta> P"
-    "TypedEqui.typed_assertion \<Delta> P" "TypedEqui.self_framing_typed \<Delta> Q" "TypedEqui.typed_assertion \<Delta> Q"
-  show "\<Delta> \<turnstile>CSL [P] Cfree r [Q \<otimes> atrue \<Delta>]"
+  assume asm0: "entails P (Q \<otimes> typed_stabilize (full_ownership r))" "TypedEqui.self_framing_typed tcfe P"
+    "TypedEqui.typed_assertion tcfe P" "TypedEqui.self_framing_typed tcfe Q" "TypedEqui.typed_assertion tcfe Q"
+  show "tcfe \<turnstile>CSL [P] Cfree r [Q \<otimes> atrue tcfe]"
   proof (rule RuleCons)
-    show "\<Delta> \<turnstile>CSL [TypedEqui.Stabilize_typed \<Delta> (full_ownership r) \<otimes> Q] Cfree r [TypedEqui.Stabilize_typed \<Delta> (atrue \<Delta>) \<otimes> Q]"
+    show "tcfe \<turnstile>CSL [TypedEqui.Stabilize_typed tcfe (full_ownership r) \<otimes> Q] Cfree r [TypedEqui.Stabilize_typed tcfe (atrue tcfe) \<otimes> Q]"
     proof (rule RuleFrame)
-      show "\<Delta> \<turnstile>CSL [TypedEqui.Stabilize_typed \<Delta> (full_ownership r)] Cfree r [TypedEqui.Stabilize_typed \<Delta> (atrue \<Delta>)]"
-        by (simp add: RuleFree RuleStabilizeTyped)
+      show "tcfe \<turnstile>CSL [TypedEqui.Stabilize_typed tcfe (full_ownership r)] Cfree r [TypedEqui.Stabilize_typed tcfe (atrue tcfe)]"
+        using RuleFree RuleStabilizeTyped by blast
     qed (simp_all add: asm0)
-    show "P \<subseteq> TypedEqui.Stabilize_typed \<Delta> (full_ownership r) \<otimes> Q"
+    show "P \<subseteq> TypedEqui.Stabilize_typed tcfe (full_ownership r) \<otimes> Q"
       by (simp add: assms helper_exhale_encoding)
-    show "TypedEqui.Stabilize_typed \<Delta> (atrue \<Delta>) \<otimes> Q \<subseteq> Q \<otimes> atrue \<Delta>"
+    show "TypedEqui.Stabilize_typed tcfe (atrue tcfe) \<otimes> Q \<subseteq> Q \<otimes> atrue tcfe"
       by (metis TypedEqui.typed_Stabilize_typed TypedEqui.typed_assertion_def add_set_commm add_set_mono TypedEqui.atrue_def mem_Collect_eq subsetI)
   qed
 qed
 
 lemma in_Stabilize_typed:
   assumes "stabilize \<omega> \<in> A"
-      and "TypedEqui.typed \<Delta> \<omega>"
-    shows "\<omega> \<in> TypedEqui.Stabilize_typed \<Delta> A"
+      and "TypedEqui.typed tcfe \<omega>"
+    shows "\<omega> \<in> TypedEqui.Stabilize_typed tcfe A"
   using ConcreteSemantics.stabilize_typed_elem assms(1) assms(2) by blast
 
 
@@ -221,51 +245,51 @@ qed
 
 
 lemma in_times_atrue:
-  assumes "TypedEqui.typed \<Delta> \<omega>'"
+  assumes "TypedEqui.typed tcfe \<omega>'"
       and "\<omega>' \<succeq> \<omega>"
       and "\<omega> \<in> A"
-    shows "\<omega>' \<in> A \<otimes> atrue \<Delta>"
+    shows "\<omega>' \<in> A \<otimes> atrue tcfe"
 proof -
   obtain r where "Some \<omega>' = \<omega> \<oplus> r"
     using assms(2) greater_def by blast
-  then have "r \<in> atrue \<Delta>"
+  then have "r \<in> atrue tcfe"
     using TypedEqui.typed_smaller assms(1) TypedEqui.atrue_def greater_equiv by blast
   then show ?thesis
     using \<open>Some \<omega>' = \<omega> \<oplus> r\<close> assms(3) x_elem_set_product by blast
 qed
 
 lemma convert_proof_write:
-  assumes "ConcreteSemantics.SL_proof \<Delta> P (Custom (FieldAssign (semantify_addr r) field_val (semantify_exp e))) Q"
-  shows "\<Delta> \<turnstile>CSL [P] Cwrite r e [Q \<otimes> atrue \<Delta>]"
+  assumes "ConcreteSemantics.SL_proof tcfe P (Custom (FieldAssign (semantify_addr r) field_val (semantify_exp e))) Q"
+  shows "tcfe \<turnstile>CSL [P] Cwrite r e [Q \<otimes> atrue tcfe]"
   using assms(1)
 proof (rule ConcreteSemantics.SL_proof_Custom_elim)
-  assume asm0: "SL_Custom \<Delta> P (custom.FieldAssign (semantify_addr r) field_val (semantify_exp e)) Q"
-  "TypedEqui.self_framing_typed \<Delta> P" "TypedEqui.typed_assertion \<Delta> P" "TypedEqui.self_framing_typed \<Delta> Q"
-  "TypedEqui.typed_assertion \<Delta> Q"
-  show "\<Delta> \<turnstile>CSL [P] Cwrite r e [Q \<otimes> atrue \<Delta>]"
+  assume asm0: "SL_Custom tcfe P (custom.FieldAssign (semantify_addr r) field_val (semantify_exp e)) Q"
+  "TypedEqui.self_framing_typed tcfe P" "TypedEqui.typed_assertion tcfe P" "TypedEqui.self_framing_typed tcfe Q"
+  "TypedEqui.typed_assertion tcfe Q"
+  show "tcfe \<turnstile>CSL [P] Cwrite r e [Q \<otimes> atrue tcfe]"
     using asm0(1)
   proof (rule SL_custom_FieldAssign)
-    assume asm1: "Q = update_value \<Delta> P (semantify_addr r) field_val (semantify_exp e)"
-      "TypedEqui.self_framing_typed \<Delta> P" "entails P {\<omega>. \<exists>l. get_m \<omega> (l, field_val) = 1 \<and> semantify_addr r \<omega> = Some l}"
+    assume asm1: "Q = update_value tcfe P (semantify_addr r) field_val (semantify_exp e)"
+      "TypedEqui.self_framing_typed tcfe P" "entails P {\<omega>. \<exists>l. get_m \<omega> (l, field_val) = 1 \<and> semantify_addr r \<omega> = Some l}"
       "framed_by_exp P (semantify_addr r)" "framed_by_exp P (semantify_exp e)"
-    show "\<Delta> \<turnstile>CSL [P] Cwrite r e [Q \<otimes> atrue \<Delta>]"
+    show "tcfe \<turnstile>CSL [P] Cwrite r e [Q \<otimes> atrue tcfe]"
     proof (rule RuleCons)
-      let ?F = "TypedEqui.Stabilize_typed \<Delta> { remove_only \<omega> (l, field_val) |\<omega> l. \<omega> \<in> P \<and> semantify_addr r \<omega> = Some l}"
-      show "\<Delta> \<turnstile>CSL [TypedEqui.Stabilize_typed \<Delta> (full_ownership r) \<otimes> ?F] Cwrite r e [TypedEqui.Stabilize_typed \<Delta> (full_ownership_with_val r e) \<otimes> ?F]"
+      let ?F = "TypedEqui.Stabilize_typed tcfe { remove_only \<omega> (l, field_val) |\<omega> l. \<omega> \<in> P \<and> semantify_addr r \<omega> = Some l}"
+      show "tcfe \<turnstile>CSL [TypedEqui.Stabilize_typed tcfe (full_ownership r) \<otimes> ?F] Cwrite r e [TypedEqui.Stabilize_typed tcfe (full_ownership_with_val r e) \<otimes> ?F]"
       proof (rule RuleFrame)
-        show "\<Delta> \<turnstile>CSL [TypedEqui.Stabilize_typed \<Delta> (full_ownership r)] Cwrite r e [TypedEqui.Stabilize_typed \<Delta> (full_ownership_with_val r e)]"
+        show "tcfe \<turnstile>CSL [TypedEqui.Stabilize_typed tcfe (full_ownership r)] Cwrite r e [TypedEqui.Stabilize_typed tcfe (full_ownership_with_val r e)]"
           by (simp add: RuleStabilizeTyped RuleWrite)
       qed (simp_all)
-      show "P \<subseteq> TypedEqui.Stabilize_typed \<Delta> (full_ownership r) \<otimes> ?F"
+      show "P \<subseteq> TypedEqui.Stabilize_typed tcfe (full_ownership r) \<otimes> ?F"
       proof
         fix \<omega> assume "\<omega> \<in> P"
         then obtain l where "get_m \<omega> (l, field_val) = 1 \<and> semantify_addr r \<omega> = Some l"          
           by (smt (verit) CollectD asm1(3) entails_def subsetD)
         then have "Some \<omega> = remove_only \<omega> (l, field_val) \<oplus> set_state \<omega> (Abs_virtual_state (concretize (\<lambda>l'. if (l, field_val) = l' then 1 else 0) (get_state \<omega>)))"
           using split_remove_only_owns_only by blast
-        moreover have "set_state \<omega> (Abs_virtual_state (concretize (\<lambda>l'. if (l, field_val) = l' then 1 else 0) (get_state \<omega>))) \<in> TypedEqui.Stabilize_typed \<Delta> (full_ownership r)"
+        moreover have "set_state \<omega> (Abs_virtual_state (concretize (\<lambda>l'. if (l, field_val) = l' then 1 else 0) (get_state \<omega>))) \<in> TypedEqui.Stabilize_typed tcfe (full_ownership r)"
         proof (rule in_Stabilize_typed)
-          show "TypedEqui.typed \<Delta> (set_state \<omega> (Abs_virtual_state (concretize (\<lambda>l'. if (l, field_val) = l' then 1 else 0) (get_state \<omega>))))"
+          show "TypedEqui.typed tcfe (set_state \<omega> (Abs_virtual_state (concretize (\<lambda>l'. if (l, field_val) = l' then 1 else 0) (get_state \<omega>))))"
             using TypedEqui.typed_state_axioms \<open>\<omega> \<in> P\<close> asm0(3) calculation greater_equiv typed_state.typed_assertionE typed_state.typed_smaller by blast
           show "stabilize (set_state \<omega> (Abs_virtual_state (concretize (\<lambda>l'. if (l, field_val) = l' then 1 else 0) (get_state \<omega>)))) \<in> full_ownership r"
             apply (rule in_full_ownership[of _ _ l])
@@ -278,16 +302,16 @@ proof (rule ConcreteSemantics.SL_proof_Custom_elim)
             by (simp add: remove_only_stabilize)
           then show "stabilize (remove_only \<omega> (l, field_val)) \<in> {remove_only \<omega> (l, field_val) |\<omega> l. \<omega> \<in> P \<and> semantify_addr r \<omega> = Some l}"
             by (smt (verit, ccfv_threshold) AbstractSemantics.get_store_stabilize CollectI TypedEqui.self_framing_typedE TypedEqui.typed_state_axioms \<open>\<omega> \<in> P\<close> \<open>get_m \<omega> (l, field_val) = 1 \<and> semantify_addr r \<omega> = Some l\<close> asm0(3) asm1(2) semantify_addr_equiv typed_state.typed_assertionE)
-          show "TypedEqui.typed \<Delta> (remove_only \<omega> (l, field_val))"
+          show "TypedEqui.typed tcfe (remove_only \<omega> (l, field_val))"
             by (meson TypedEqui.typed_assertion_def TypedEqui.typed_state_axioms \<open>\<omega> \<in> P\<close> asm0(3) calculation(1) greater_def typed_state.typed_smaller)
         qed
-        ultimately show "\<omega> \<in> TypedEqui.Stabilize_typed \<Delta> (full_ownership r) \<otimes> ?F"
+        ultimately show "\<omega> \<in> TypedEqui.Stabilize_typed tcfe (full_ownership r) \<otimes> ?F"
           using commutative x_elem_set_product by fastforce
       qed
-      show "TypedEqui.Stabilize_typed \<Delta> (full_ownership_with_val r e) \<otimes> ?F \<subseteq> Q \<otimes> atrue \<Delta>"
+      show "TypedEqui.Stabilize_typed tcfe (full_ownership_with_val r e) \<otimes> ?F \<subseteq> Q \<otimes> atrue tcfe"
       proof
-        fix \<omega>' assume "\<omega>' \<in> TypedEqui.Stabilize_typed \<Delta> (full_ownership_with_val r e) \<otimes> ?F"
-        then obtain ptr f where r: "Some \<omega>' = ptr \<oplus> f" "ptr \<in> TypedEqui.Stabilize_typed \<Delta> (full_ownership_with_val r e)" "f \<in> ?F"
+        fix \<omega>' assume "\<omega>' \<in> TypedEqui.Stabilize_typed tcfe (full_ownership_with_val r e) \<otimes> ?F"
+        then obtain ptr f where r: "Some \<omega>' = ptr \<oplus> f" "ptr \<in> TypedEqui.Stabilize_typed tcfe (full_ownership_with_val r e)" "f \<in> ?F"
           by (meson x_elem_set_product)
         then obtain l where "get_store (stabilize ptr) r = Some (VRef (Address l)) \<and> get_m (stabilize ptr) (l, field_val) = 1
   \<and> get_h (stabilize ptr) (l, field_val) = Some (VInt (edenot e (get_store (stabilize ptr))))"
@@ -328,11 +352,17 @@ proof (rule ConcreteSemantics.SL_proof_Custom_elim)
           show "get_trace \<omega>' = get_trace (update_heap_val \<omega> (l, field_val) (VInt (edenot e (get_store \<omega>'))))"
             by (metis \<open>stabilize f = remove_only \<omega> (l', field_val)\<close> get_trace_set_state get_trace_stabilize greater_equiv greater_state_has_greater_parts(2) r(1) remove_only_def)
         qed
+
+
         moreover have "update_heap_val \<omega> (l, field_val) (VInt (edenot e (get_store \<omega>'))) \<in> Q"
           using \<open>l = l'\<close>
+          sorry
+(*
+
           by (smt (verit, ccfv_SIG) AbstractSemantics.get_store_stabilize ConcreteSemantics.stabilize_typed_elem \<open>\<omega> \<in> P\<close> \<open>get_store ptr r = Some (VRef (Address l)) \<and> get_m ptr (l, field_val) = 1 \<and> get_h ptr (l, field_val) = Some (VInt (edenot e (get_store ptr)))\<close> \<open>semantify_addr r \<omega> = Some l'\<close> \<open>stabilize f = remove_only \<omega> (l', field_val)\<close> asm1(1) full_add_charact(1) full_add_defined get_store_set_state in_update_value r(1) r(2) remove_only_def semantify_exp_def snd_conv typed_get_vh)
-        ultimately show "\<omega>' \<in> Q \<otimes> atrue \<Delta>"
-          by (meson TypedEqui.typed_assertionE TypedEqui.typed_state_axioms \<open>\<omega>' \<in> TypedEqui.Stabilize_typed \<Delta> (full_ownership_with_val r e) \<otimes> TypedEqui.Stabilize_typed \<Delta> {remove_only \<omega> (l, field_val) |\<omega> l. \<omega> \<in> P \<and> semantify_addr r \<omega> = Some l}\<close> in_times_atrue typed_state.typed_Stabilize_typed typed_state.typed_star)
+*)
+        ultimately show "\<omega>' \<in> Q \<otimes> atrue tcfe"
+          by (meson TypedEqui.typed_assertionE TypedEqui.typed_state_axioms \<open>\<omega>' \<in> TypedEqui.Stabilize_typed tcfe (full_ownership_with_val r e) \<otimes> TypedEqui.Stabilize_typed tcfe {remove_only \<omega> (l, field_val) |\<omega> l. \<omega> \<in> P \<and> semantify_addr r \<omega> = Some l}\<close> in_times_atrue typed_state.typed_Stabilize_typed typed_state.typed_star)
       qed
     qed
   qed
@@ -346,14 +376,13 @@ definition semantify_heap_loc :: "var \<Rightarrow> (int equi_state, int val) Ab
   else None)"
 
 lemma convert_proof_read:
-  assumes "ConcreteSemantics.SL_proof \<Delta> P (LocalAssign x (semantify_heap_loc r)) Q"
-      and "custom_context \<Delta> = type_ctxt_heap"
-  shows "\<Delta> \<turnstile>CSL [P] Cread x r [Q]"
+  assumes "ConcreteSemantics.SL_proof tcfe P (LocalAssign x (semantify_heap_loc r)) Q"
+  shows "tcfe \<turnstile>CSL [P] Cread x r [Q]"
   using assms(1)
 proof (rule ConcreteSemantics.SL_proof_LocalAssign_elim)
   assume asm0: "Q = ConcreteSemantics.post_substitute_var_assert x (semantify_heap_loc r) P"
     "framed_by_exp P (semantify_heap_loc r)"
-    "TypedEqui.self_framing_typed \<Delta> P" "TypedEqui.typed_assertion \<Delta> P"
+    "TypedEqui.self_framing_typed tcfe P" "TypedEqui.typed_assertion tcfe P"
 
   have r: "\<And>\<omega>. \<omega> \<in> P \<Longrightarrow> (\<exists>l. get_store \<omega> r = Some (VRef (Address l)) \<and> get_m \<omega> (l, field_val) > 0
   \<and> (\<exists>v. get_h \<omega> (l, field_val) = Some (VInt v)))"
@@ -363,9 +392,9 @@ proof (rule ConcreteSemantics.SL_proof_LocalAssign_elim)
     then obtain l v0 where "get_store \<omega> r = Some (VRef (Address l))" "get_h \<omega> (l, field_val) = Some v0"
       by (metis asm0(2) framed_by_exp_def semantify_heap_loc_def)
     then obtain v where "v0 = VInt v"
-      using TypedEqui.typed_assertionE[OF asm0(4) asm1] TypedEqui.typed_def[of \<Delta> \<omega>] well_typedE(1)[of "custom_context \<Delta>" "get_abs_state \<omega>"]
-      Instantiation.well_typed_heapE[of "custom_context \<Delta>" "get_state \<omega>" "(l, field_val)" v0]
-      by (smt (verit, best) CollectD assms(2) option.sel snd_conv snd_get_abs_state type_ctxt_heap_def vints_def)
+      using TypedEqui.typed_assertionE[OF asm0(4) asm1] TypedEqui.typed_def[of tcfe \<omega>] well_typedE(1)[of "custom_context tcfe" "get_abs_state \<omega>"]
+      Instantiation.well_typed_heapE[of "custom_context tcfe" "get_state \<omega>" "(l, field_val)" v0]
+      by (smt (verit, del_insts) CollectD abs_type_context.select_convs(2) option.sel snd_conv snd_get_abs_state type_ctxt_front_end_def type_ctxt_heap_def vints_def)
     moreover have "stabilize \<omega> \<in> P"
       using TypedEqui.self_framing_typedE TypedEqui.typed_state_axioms \<open>\<omega> \<in> P\<close> asm0(3) asm0(4) typed_state.typed_assertionE by blast
     then have "get_h (stabilize \<omega>) (l, field_val) = Some (VInt v)"
@@ -377,9 +406,9 @@ proof (rule ConcreteSemantics.SL_proof_LocalAssign_elim)
       by (simp add: \<open>get_h \<omega> (l, field_val) = Some v0\<close> \<open>get_store \<omega> r = Some (VRef (Address l))\<close> calculation)
   qed
 
-  show "\<Delta> \<turnstile>CSL [P] Cread x r [Q]"
+  show "tcfe \<turnstile>CSL [P] Cread x r [Q]"
   proof (rule RuleCons)
-    show "\<Delta> \<turnstile>CSL [P] Cread x r [read_result P x r]"
+    show "tcfe \<turnstile>CSL [P] Cread x r [read_result P x r]"
     proof (rule RuleRead)
       show "P \<subseteq> read_perm r" (* Should come from framed_by_exp *)
         using r
@@ -402,182 +431,184 @@ proof (rule ConcreteSemantics.SL_proof_LocalAssign_elim)
   qed (simp)
 qed
 
-
-
 fun translate (* :: "cmd \<Rightarrow> (v_stmt \<times> v_stmt set)" *) where
-  "translate \<Gamma> F Cskip = (Skip, {})"
-| "translate \<Gamma> F (Cassign x e) = (LocalAssign x (semantify_exp e), {})"
+  "translate \<Gamma> Cskip = (Skip, {})"
+| "translate \<Gamma> (Cassign x e) = (LocalAssign x (semantify_exp e), {})"
 
-| "translate \<Gamma> F (Calloc r e) = ((Havoc r;; Inhale (full_ownership_with_val r e)), {})"
-| "translate \<Gamma> F (Cfree r) = (Exhale (Stabilize (full_ownership r)), {})"
-| "translate \<Gamma> F (Cwrite r e) = (Custom (FieldAssign (semantify_addr r) field_val (semantify_exp e)), {})"
-| "translate \<Gamma> F (Cread x r) = (LocalAssign x (semantify_heap_loc r), {})"
+| "translate \<Gamma> (Calloc r e) = ((Havoc r;; Inhale (typed_stabilize (full_ownership_with_val r e))), {})"
+| "translate \<Gamma> (Cfree r) = (Exhale (typed_stabilize (full_ownership r)), {})"
+| "translate \<Gamma> (Cwrite r e) = (Custom (FieldAssign (semantify_addr r) field_val (semantify_exp e)), {})"
+| "translate \<Gamma> (Cread x r) = (LocalAssign x (semantify_heap_loc r), {})"
 
-| "translate \<Gamma> F (Cseq C1 C2) = (let r1 = translate \<Gamma> F C1 in let r2 = translate \<Gamma> F C2 in
+| "translate \<Gamma> (Cseq C1 C2) = (let r1 = translate \<Gamma> C1 in let r2 = translate \<Gamma> C2 in
   (fst r1;; fst r2, snd r1 \<union> snd r2))"
 
-| "translate \<Gamma> F (Cif b C1 C2) = (If (semantify_bexp b) (fst (translate \<Gamma> F C1)) (fst (translate \<Gamma> F C2)), snd (translate \<Gamma> F C1) \<union> snd (translate \<Gamma> F C2))"
+| "translate \<Gamma> (Cif b C1 C2) = (If (semantify_bexp b) (fst (translate \<Gamma> C1)) (fst (translate \<Gamma> C2)), snd (translate \<Gamma> C1) \<union> snd (translate \<Gamma> C2))"
 
-| "translate \<Gamma> F ({P1} C1 {Q1} || {P2} C2 {Q2}) =
-  ((Exhale (make_semantic_assertion \<Gamma> F P1 \<otimes> make_semantic_assertion \<Gamma> F P2);;
+| "translate \<Gamma> ({P1} C1 {Q1} || {P2} C2 {Q2}) =
+  ((Exhale (make_semantic_assertion \<Gamma> type_ctxt_front_end_syntactic P1 \<otimes> make_semantic_assertion \<Gamma> type_ctxt_front_end_syntactic P2);;
   ConcreteSemantics.havoc_list (wrL C1 @ wrL C2);;
-  Inhale (make_semantic_assertion \<Gamma> F Q1 \<otimes> make_semantic_assertion \<Gamma> F Q2)),
-  let r1 = translate \<Gamma> F C1 in let r2 = translate \<Gamma> F C2 in
-  { (Inhale (make_semantic_assertion \<Gamma> F P1);; fst r1;; Exhale (make_semantic_assertion \<Gamma> F Q1)),
-  (Inhale (make_semantic_assertion \<Gamma> F P2);; fst r2;; Exhale (make_semantic_assertion \<Gamma> F Q2)) } \<union> snd r1 \<union> snd r2)"
+  Inhale (make_semantic_assertion \<Gamma> type_ctxt_front_end_syntactic Q1 \<otimes> make_semantic_assertion \<Gamma> type_ctxt_front_end_syntactic Q2)),
+  let r1 = translate \<Gamma> C1 in let r2 = translate \<Gamma> C2 in
+  { (Inhale (make_semantic_assertion \<Gamma> type_ctxt_front_end_syntactic P1);; fst r1;; Exhale (make_semantic_assertion \<Gamma> type_ctxt_front_end_syntactic Q1)),
+  (Inhale (make_semantic_assertion \<Gamma> type_ctxt_front_end_syntactic P2);; fst r2;; Exhale (make_semantic_assertion \<Gamma> type_ctxt_front_end_syntactic Q2)) } \<union> snd r1 \<union> snd r2)"
 
-| "translate \<Gamma> F (Cwhile b I C) = (Exhale (make_semantic_assertion \<Gamma> F I);;
-  ConcreteSemantics.havoc_list (wrL C);; Inhale ((make_semantic_assertion \<Gamma> F I) \<inter> assertify_bexp (Bnot b)),
-  { Inhale ((make_semantic_assertion \<Gamma> F I) \<inter> assertify_bexp b);; fst (translate \<Gamma> F C);; Exhale (make_semantic_assertion \<Gamma> F I) } \<union> snd (translate \<Gamma> F C))"
+| "translate \<Gamma> (Cwhile b I C) = (Exhale (make_semantic_assertion \<Gamma> type_ctxt_front_end_syntactic I);;
+  ConcreteSemantics.havoc_list (wrL C);; Inhale ((make_semantic_assertion \<Gamma> type_ctxt_front_end_syntactic I) \<inter> assertify_bexp (Bnot b)),
+  { Inhale ((make_semantic_assertion \<Gamma> type_ctxt_front_end_syntactic I) \<inter> assertify_bexp b);; fst (translate \<Gamma> C);; Exhale (make_semantic_assertion \<Gamma> type_ctxt_front_end_syntactic I) } \<union> snd (translate \<Gamma> C))"
 
 lemma CSL_weaken_post_atrue:
-  assumes "\<Delta> \<turnstile>CSL [P] C [Q]"
-      and "TypedEqui.typed_assertion \<Delta> Q"
-  shows "\<Delta> \<turnstile>CSL [P] C [Q \<otimes> atrue \<Delta>]"
+  assumes "tcfe \<turnstile>CSL [P] C [Q]"
+      and "TypedEqui.typed_assertion tcfe Q"
+  shows "tcfe \<turnstile>CSL [P] C [Q \<otimes> atrue tcfe]"
   using assms(1)
 proof (rule RuleCons)
-  show "Q \<subseteq> Q \<otimes> atrue \<Delta>"
+  show "Q \<subseteq> Q \<otimes> atrue tcfe"
     using add_set_commm assms(2) conjunct_with_true_entails by blast
 qed (simp)
 
 lemma CSL_add_atrue:
-  assumes "\<Delta> \<turnstile>CSL [P] C [Q]"
-      and "TypedEqui.self_framing_typed \<Delta> P"
-      and "TypedEqui.typed_assertion \<Delta> P"
-      and "TypedEqui.wf_context \<Delta>"
-    shows "\<Delta> \<turnstile>CSL [P \<otimes> atrue \<Delta>] C [Q \<otimes> atrue \<Delta>]"
+  assumes "tcfe \<turnstile>CSL [P] C [Q]"
+      and "TypedEqui.self_framing_typed tcfe P"
+      and "TypedEqui.typed_assertion tcfe P"
+      and "TypedEqui.wf_context tcfe"
+    shows "tcfe \<turnstile>CSL [P \<otimes> atrue tcfe] C [Q \<otimes> atrue tcfe]"
   by (rule RuleFrame) (simp_all add: assms)
 
 
 definition proof_obligations_valid where
-  "proof_obligations_valid \<Delta> S \<longleftrightarrow> (\<forall>Cv \<in> S. \<exists>B. ConcreteSemantics.SL_proof \<Delta> (atrue \<Delta>) Cv B)"
+  "proof_obligations_valid S \<longleftrightarrow> (\<forall>Cv \<in> S. \<exists>B. ConcreteSemantics.SL_proof tcfe (atrue tcfe) Cv B)"
 
 lemma proof_obligations_valid_union:
-  "proof_obligations_valid \<Delta> (S1 \<union> S2) \<longleftrightarrow> proof_obligations_valid \<Delta> S1 \<and> proof_obligations_valid \<Delta> S2"
+  "proof_obligations_valid (S1 \<union> S2) \<longleftrightarrow> proof_obligations_valid S1 \<and> proof_obligations_valid S2"
   by (meson Un_iff proof_obligations_valid_def)
 
 definition invariant_translate where
-  "invariant_translate \<Gamma> F \<Delta> P C Q \<longleftrightarrow>
-  ((proof_obligations_valid \<Delta> (snd (translate \<Gamma> F C)) \<and> ConcreteSemantics.SL_proof \<Delta> P (fst (translate \<Gamma> F C)) Q) \<longrightarrow> \<Delta> \<turnstile>CSL [P \<otimes> atrue \<Delta>] C [Q \<otimes> atrue \<Delta>])"
+  "invariant_translate \<Gamma> P C Q \<longleftrightarrow>
+  ((proof_obligations_valid (snd (translate \<Gamma> C)) \<and> ConcreteSemantics.SL_proof tcfe P (fst (translate \<Gamma> C)) Q) \<longrightarrow> tcfe \<turnstile>CSL [P \<otimes> atrue tcfe] C [Q \<otimes> atrue tcfe])"
 
 lemma invariant_translateE:
-  assumes "invariant_translate \<Gamma> F \<Delta> P C Q"
-      and "proof_obligations_valid \<Delta> (snd (translate \<Gamma> F C))"
-      and "ConcreteSemantics.SL_proof \<Delta> P (fst (translate \<Gamma> F C)) Q"
-    shows "\<Delta> \<turnstile>CSL [P \<otimes> atrue \<Delta>] C [Q \<otimes> atrue \<Delta>]"
+  assumes "invariant_translate \<Gamma> P C Q"
+      and "proof_obligations_valid (snd (translate \<Gamma> C))"
+      and "ConcreteSemantics.SL_proof tcfe P (fst (translate \<Gamma> C)) Q"
+    shows "tcfe \<turnstile>CSL [P \<otimes> atrue tcfe] C [Q \<otimes> atrue tcfe]"
   using assms(1) assms(2) assms(3) invariant_translate_def by blast
 
 
 lemma invariant_translateI:
-  assumes "proof_obligations_valid \<Delta> (snd (translate \<Gamma> F C)) \<Longrightarrow> ConcreteSemantics.SL_proof \<Delta> P (fst (translate \<Gamma> F C)) Q
-    \<Longrightarrow> \<Delta> \<turnstile>CSL [P \<otimes> atrue \<Delta>] C [Q \<otimes> atrue \<Delta>]"
-  shows "invariant_translate \<Gamma> F \<Delta> P C Q"
+  assumes "proof_obligations_valid (snd (translate \<Gamma> C)) \<Longrightarrow> ConcreteSemantics.SL_proof tcfe P (fst (translate \<Gamma> C)) Q
+    \<Longrightarrow> tcfe \<turnstile>CSL [P \<otimes> atrue tcfe] C [Q \<otimes> atrue tcfe]"
+  shows "invariant_translate \<Gamma> P C Q"
   using assms invariant_translate_def proof_obligations_valid_def by blast
 
 lemma invariant_translate_simpler:
-  assumes "ConcreteSemantics.SL_proof \<Delta> P (fst (translate \<Gamma> F C)) Q \<Longrightarrow> \<Delta> \<turnstile>CSL [P] C [Q]"
-      and "ConcreteSemantics.wf_abs_stmt \<Delta> (fst (translate \<Gamma> F C))"
-      and "TypedEqui.wf_context \<Delta>"
-    shows "invariant_translate \<Gamma> F \<Delta> P C Q"
+  assumes "ConcreteSemantics.SL_proof tcfe P (fst (translate \<Gamma> C)) Q \<Longrightarrow> tcfe \<turnstile>CSL [P] C [Q]"
+      and "ConcreteSemantics.wf_abs_stmt tcfe (fst (translate \<Gamma> C))"
+      and "TypedEqui.wf_context tcfe"
+    shows "invariant_translate \<Gamma> P C Q"
   by (simp add: CSL_add_atrue ConcreteSemantics.proofs_are_self_framing_and_typed assms invariant_translateI)
 
 corollary invariant_translate_skip:
-  assumes "TypedEqui.wf_context \<Delta>"
-  shows "invariant_translate \<Gamma> F \<Delta> P Cskip Q"
-  using convert_proof_skip invariant_translate_simpler assms by fastforce
+  assumes "TypedEqui.wf_context tcfe"
+  shows "invariant_translate \<Gamma> P Cskip Q"
+  using convert_proof_skip invariant_translate_simpler assms  
+  by (metis ConcreteSemantics.wf_abs_stmt.simps(1) fst_eqD translate.simps(1))
 
 corollary invariant_translate_assign:
-  assumes "ConcreteSemantics.wf_abs_stmt \<Delta> (fst (translate \<Gamma> F (Cassign x e)))"
-      and "TypedEqui.wf_context \<Delta>"
-    shows "invariant_translate \<Gamma> F \<Delta> P (Cassign x e) Q"
-  using convert_proof_assign invariant_translate_simpler assms by fastforce
+  assumes "ConcreteSemantics.wf_abs_stmt tcfe (fst (translate \<Gamma> (Cassign x e)))"
+      and "TypedEqui.wf_context tcfe"
+    shows "invariant_translate \<Gamma> P (Cassign x e) Q"
+  using convert_proof_assign invariant_translate_simpler assms
+  by (metis fst_eqD translate.simps(2))
+
 
 corollary invariant_translate_alloc:
-  assumes "well_typed_cmd \<Delta> (Calloc r e)"
-      and "wf_stmt \<Gamma> F \<Delta> (Calloc r e)"
-      and "ConcreteSemantics.wf_abs_stmt \<Delta> (fst (translate \<Gamma> F (Calloc r e)))"
-      and "TypedEqui.wf_context \<Delta>"
-    shows "invariant_translate \<Gamma> F \<Delta> P (Calloc r e) Q"
-  using assms cmd.distinct(37) convert_proof_alloc invariant_translate_simpler by fastforce
+  assumes "well_typed_cmd tcfe (Calloc r e)"
+      and "wf_stmt \<Gamma> type_ctxt_front_end_syntactic (Calloc r e)"
+      and "ConcreteSemantics.wf_abs_stmt tcfe (fst (translate \<Gamma> (Calloc r e)))"
+    shows "invariant_translate \<Gamma> P (Calloc r e) Q"
+  using assms cmd.distinct(37) convert_proof_alloc invariant_translate_simpler
+  by (metis fst_eqD translate.simps(3) wf_context_type_context)
 
 lemma atrue_twice_same:
-  "atrue \<Delta> \<otimes> atrue \<Delta> \<subseteq> atrue \<Delta>"
+  "atrue tcfe \<otimes> atrue tcfe \<subseteq> atrue tcfe"
   unfolding TypedEqui.atrue_def add_set_def
   by (smt (z3) Collect_mono_iff TypedEqui.typed_sum mem_Collect_eq)
 
 lemma atrue_twice_equal:
-  "atrue \<Delta> \<otimes> atrue \<Delta> = atrue \<Delta>"
+  "atrue tcfe \<otimes> atrue tcfe = atrue tcfe"
 proof
-  show "atrue \<Delta> \<subseteq> atrue \<Delta> \<otimes> atrue \<Delta>"
+  show "atrue tcfe \<subseteq> atrue tcfe \<otimes> atrue tcfe"
   proof
-    fix x assume "x \<in> atrue \<Delta>"
+    fix x assume "x \<in> atrue tcfe"
     then have "Some x = x \<oplus> |x|"
       using core_is_smaller by blast
-    then have "|x| \<in> atrue \<Delta>"
-      using TypedEqui.typed_core \<open>x \<in> atrue \<Delta>\<close> TypedEqui.atrue_def by blast
-    then show "x \<in> atrue \<Delta> \<otimes> atrue \<Delta>"
-      using \<open>Some x = x \<oplus> |x|\<close> \<open>x \<in> atrue \<Delta>\<close> x_elem_set_product by blast
+    then have "|x| \<in> atrue tcfe"
+      using TypedEqui.typed_core \<open>x \<in> atrue tcfe\<close> TypedEqui.atrue_def by blast
+    then show "x \<in> atrue tcfe \<otimes> atrue tcfe"
+      using \<open>Some x = x \<oplus> |x|\<close> \<open>x \<in> atrue tcfe\<close> x_elem_set_product by blast
   qed
 qed (simp add: atrue_twice_same)
 
 
 corollary invariant_translate_free:
-  assumes "ConcreteSemantics.wf_abs_stmt \<Delta> (fst (translate \<Gamma> F (Cfree r)))"
-      and "TypedEqui.wf_context \<Delta>"
-    shows "invariant_translate \<Gamma> F \<Delta> P (Cfree r) Q"
+  assumes "ConcreteSemantics.wf_abs_stmt tcfe (fst (translate \<Gamma> (Cfree r)))"
+      and "TypedEqui.wf_context tcfe"
+    shows "invariant_translate \<Gamma> P (Cfree r) Q"
 proof (rule invariant_translateI)
-  assume asm0: "ConcreteSemantics.SL_proof \<Delta> P (fst (translate \<Gamma> F (Cfree r))) Q"
-  then have "\<Delta> \<turnstile>CSL [P \<otimes> atrue \<Delta>] Cfree r [(Q \<otimes> atrue \<Delta>) \<otimes> atrue \<Delta>]"
+  assume asm0: "ConcreteSemantics.SL_proof tcfe P (fst (translate \<Gamma> (Cfree r))) Q"
+  then have "tcfe \<turnstile>CSL [P \<otimes> atrue tcfe] Cfree r [(Q \<otimes> atrue tcfe) \<otimes> atrue tcfe]"
     using RuleFrame[OF convert_proof_free]
     by (metis CSL_add_atrue ConcreteSemantics.proofs_are_self_framing_and_typed assms convert_proof_free fst_eqD translate.simps(4))
-  then show "\<Delta> \<turnstile>CSL [P \<otimes> atrue \<Delta>] Cfree r [Q \<otimes> atrue \<Delta>]"
+  then show "tcfe \<turnstile>CSL [P \<otimes> atrue tcfe] Cfree r [Q \<otimes> atrue tcfe]"
     by (simp add: add_set_asso atrue_twice_equal)
 qed
 
 corollary invariant_translate_write:
-  assumes "ConcreteSemantics.wf_abs_stmt \<Delta> (fst (translate \<Gamma> F (Cwrite r e)))"
-      and "TypedEqui.wf_context \<Delta>"
-    shows "invariant_translate \<Gamma> F \<Delta> P (Cwrite r e) Q"
+  assumes "ConcreteSemantics.wf_abs_stmt tcfe (fst (translate \<Gamma> (Cwrite r e)))"
+      and "TypedEqui.wf_context tcfe"
+    shows "invariant_translate \<Gamma> P (Cwrite r e) Q"
 proof (rule invariant_translateI)
-  assume asm0: "ConcreteSemantics.SL_proof \<Delta> P (fst (translate \<Gamma> F (Cwrite r e))) Q"
-  then have "\<Delta> \<turnstile>CSL [P \<otimes> atrue \<Delta>] Cwrite r e [(Q \<otimes> atrue \<Delta>) \<otimes> atrue \<Delta>]"
+  assume asm0: "ConcreteSemantics.SL_proof tcfe P (fst (translate \<Gamma> (Cwrite r e))) Q"
+  then have "tcfe \<turnstile>CSL [P \<otimes> atrue tcfe] Cwrite r e [(Q \<otimes> atrue tcfe) \<otimes> atrue tcfe]"
     using RuleFrame[OF convert_proof_write]
     by (metis CSL_add_atrue ConcreteSemantics.proofs_are_self_framing_and_typed assms convert_proof_write fst_eqD translate.simps(5))
-  then show "\<Delta> \<turnstile>CSL [P \<otimes> atrue \<Delta>] Cwrite r e [Q \<otimes> atrue \<Delta>]"
+  then show "tcfe \<turnstile>CSL [P \<otimes> atrue tcfe] Cwrite r e [Q \<otimes> atrue tcfe]"
     by (simp add: add_set_asso atrue_twice_equal)
 qed
 
 corollary invariant_translate_read:
-  assumes "ConcreteSemantics.wf_abs_stmt \<Delta> (fst (translate \<Gamma> F (Cread x r)))"
-      and "TypedEqui.wf_context \<Delta>"
-      and "custom_context \<Delta> = type_ctxt_heap"
-    shows "invariant_translate \<Gamma> F \<Delta> P (Cread x r) Q"
-  using convert_proof_read invariant_translate_simpler assms by fastforce
+  assumes "ConcreteSemantics.wf_abs_stmt tcfe (fst (translate \<Gamma> (Cread x r)))"
+      and "TypedEqui.wf_context tcfe"
+      and "custom_context tcfe = type_ctxt_heap"
+    shows "invariant_translate \<Gamma> P (Cread x r) Q"
+  using convert_proof_read invariant_translate_simpler assms
+  by (metis fst_eqD translate.simps(6))
 
 
 lemma invariant_translate_seq:
-  assumes "\<And>R. invariant_translate \<Gamma> F \<Delta> P C1 R"
-      and "\<And>R. invariant_translate \<Gamma> F \<Delta> R C2 Q"
-    shows "invariant_translate \<Gamma> F \<Delta> P (Cseq C1 C2) Q"
+  assumes "\<And>R. invariant_translate \<Gamma> P C1 R"
+      and "\<And>R. invariant_translate \<Gamma> R C2 Q"
+    shows "invariant_translate \<Gamma> P (Cseq C1 C2) Q"
 proof (rule invariant_translateI)
-  assume asm0: "proof_obligations_valid \<Delta> (snd (translate \<Gamma> F (Cseq C1 C2)))"
-    "ConcreteSemantics.SL_proof \<Delta> P (fst (translate \<Gamma> F (Cseq C1 C2))) Q"
-  then obtain R where r: "ConcreteSemantics.SL_proof \<Delta> P (fst (translate \<Gamma> F C1)) R"
-      "ConcreteSemantics.SL_proof \<Delta> R (fst (translate \<Gamma> F C2)) Q"
+  assume asm0: "proof_obligations_valid (snd (translate \<Gamma> (Cseq C1 C2)))"
+    "ConcreteSemantics.SL_proof tcfe P (fst (translate \<Gamma> (Cseq C1 C2))) Q"
+  then obtain R where r: "ConcreteSemantics.SL_proof tcfe P (fst (translate \<Gamma> C1)) R"
+      "ConcreteSemantics.SL_proof tcfe R (fst (translate \<Gamma> C2)) Q"
     by (metis ConcreteSemantics.SL_proof_Seq_elim fst_eqD translate.simps(7))
-  show "\<Delta> \<turnstile>CSL [P \<otimes> atrue \<Delta>] Cseq C1 C2 [Q \<otimes> atrue \<Delta>]"
+  show "tcfe \<turnstile>CSL [P \<otimes> atrue tcfe] Cseq C1 C2 [Q \<otimes> atrue tcfe]"
   proof (rule RuleSeq)
-    show "\<Delta> \<turnstile>CSL [P \<otimes> atrue \<Delta>] C1 [R \<otimes> atrue \<Delta>]"
+    show "tcfe \<turnstile>CSL [P \<otimes> atrue tcfe] C1 [R \<otimes> atrue tcfe]"
       using assms(1)[of R] r
       unfolding invariant_translate_def
       by (metis asm0(1) proof_obligations_valid_union snd_conv translate.simps(7))
-    show "\<Delta> \<turnstile>CSL [R \<otimes> atrue \<Delta>] C2 [Q \<otimes> atrue \<Delta>]"
+    show "tcfe \<turnstile>CSL [R \<otimes> atrue tcfe] C2 [Q \<otimes> atrue tcfe]"
     proof (rule RuleCons)
-      show "\<Delta> \<turnstile>CSL [R \<otimes> atrue \<Delta>] C2 [(Q \<otimes> atrue \<Delta>) \<otimes> atrue \<Delta>]"
+      show "tcfe \<turnstile>CSL [R \<otimes> atrue tcfe] C2 [(Q \<otimes> atrue tcfe) \<otimes> atrue tcfe]"
           using assms(2)[of R] asm0
           unfolding invariant_translate_def proof_obligations_valid_def
           by (metis (no_types, lifting) Un_iff add_set_asso atrue_twice_equal r(2) snd_conv translate.simps(7))
-      show "Q \<otimes> atrue \<Delta> \<otimes> atrue \<Delta> \<subseteq> Q \<otimes> atrue \<Delta>"
+      show "Q \<otimes> atrue tcfe \<otimes> atrue tcfe \<subseteq> Q \<otimes> atrue tcfe"
         by (simp add: add_set_asso add_set_mono atrue_twice_same)
     qed (simp)
   qed
@@ -585,26 +616,26 @@ qed
 
 
 lemma invariant_translate_inhale_exhale_get_proof:
-  assumes "\<And>P Q. invariant_translate \<Gamma> F \<Delta> P C Q"
-      and "ConcreteSemantics.SL_proof \<Delta> P (Inhale A;; fst (translate \<Gamma> F C);; Exhale B) Q"
-      and "proof_obligations_valid \<Delta> (snd (translate \<Gamma> F C))"
-    shows "\<Delta> \<turnstile>CSL [P \<otimes> A \<otimes> atrue \<Delta>] C [Q \<otimes> B \<otimes> atrue \<Delta>]"
+  assumes "\<And>P Q. invariant_translate \<Gamma> P C Q"
+      and "ConcreteSemantics.SL_proof tcfe P (Inhale A;; fst (translate \<Gamma> C);; Exhale B) Q"
+      and "proof_obligations_valid (snd (translate \<Gamma> C))"
+    shows "tcfe \<turnstile>CSL [P \<otimes> A \<otimes> atrue tcfe] C [Q \<otimes> B \<otimes> atrue tcfe]"
   using assms(2)
 proof (rule ConcreteSemantics.SL_proof_Seq_elim)
-  fix R1 assume asm0: "ConcreteSemantics.SL_proof \<Delta> P (abs_stmt.Inhale A ;; fst (translate \<Gamma> F C)) R1"
-    "ConcreteSemantics.SL_proof \<Delta> R1 (abs_stmt.Exhale B) Q"
+  fix R1 assume asm0: "ConcreteSemantics.SL_proof tcfe P (abs_stmt.Inhale A ;; fst (translate \<Gamma> C)) R1"
+    "ConcreteSemantics.SL_proof tcfe R1 (abs_stmt.Exhale B) Q"
   then have "entails R1 (Q \<otimes> B)" by auto
-  show "\<Delta> \<turnstile>CSL [P \<otimes> A \<otimes> atrue \<Delta>] C [Q \<otimes> B \<otimes> atrue \<Delta>]"
+  show "tcfe \<turnstile>CSL [P \<otimes> A \<otimes> atrue tcfe] C [Q \<otimes> B \<otimes> atrue tcfe]"
   proof (rule ConcreteSemantics.SL_proof_Seq_elim[OF asm0(1)])
-    fix R0 assume asm1: "ConcreteSemantics.SL_proof \<Delta> P (abs_stmt.Inhale A) R0"
-          "ConcreteSemantics.SL_proof \<Delta> R0 (fst (translate \<Gamma> F C)) R1"
-    then have "ConcreteSemantics.SL_proof \<Delta> (P \<otimes> A) (fst (translate \<Gamma> F C)) R1"
+    fix R0 assume asm1: "ConcreteSemantics.SL_proof tcfe P (abs_stmt.Inhale A) R0"
+          "ConcreteSemantics.SL_proof tcfe R0 (fst (translate \<Gamma> C)) R1"
+    then have "ConcreteSemantics.SL_proof tcfe (P \<otimes> A) (fst (translate \<Gamma> C)) R1"
       by auto
-    show "\<Delta> \<turnstile>CSL [P \<otimes> A \<otimes> atrue \<Delta>] C [Q \<otimes> B \<otimes> atrue \<Delta>]"
+    show "tcfe \<turnstile>CSL [P \<otimes> A \<otimes> atrue tcfe] C [Q \<otimes> B \<otimes> atrue tcfe]"
     proof (rule RuleCons)
-      show "\<Delta> \<turnstile>CSL [P \<otimes> A \<otimes> atrue \<Delta>] C [R1 \<otimes> atrue \<Delta>]"
-        using \<open>ConcreteSemantics.SL_proof \<Delta> (P \<otimes> A) (fst (translate \<Gamma> F C)) R1\<close> assms(1) assms(3) invariant_translate_def by blast
-      show "R1 \<otimes> atrue \<Delta> \<subseteq> Q \<otimes> B \<otimes> atrue \<Delta>"
+      show "tcfe \<turnstile>CSL [P \<otimes> A \<otimes> atrue tcfe] C [R1 \<otimes> atrue tcfe]"
+        using \<open>ConcreteSemantics.SL_proof tcfe (P \<otimes> A) (fst (translate \<Gamma> C)) R1\<close> assms(1) assms(3) invariant_translate_def by blast
+      show "R1 \<otimes> atrue tcfe \<subseteq> Q \<otimes> B \<otimes> atrue tcfe"
         by (meson \<open>entails R1 (Q \<otimes> B)\<close> add_set_mono entails_def order_refl)
     qed (simp)
   qed
@@ -612,25 +643,26 @@ qed
 
 
 lemma drop_conjunct_entails:
-  assumes "TypedEqui.typed_assertion \<Delta> A"
-  shows "A \<otimes> B \<otimes> atrue \<Delta> \<subseteq> B \<otimes> atrue \<Delta>"
+  assumes "TypedEqui.typed_assertion tcfe A"
+  shows "A \<otimes> B \<otimes> atrue tcfe \<subseteq> B \<otimes> atrue tcfe"
   by (smt (verit) TypedEqui.typed_assertion_def add_set_asso add_set_commm add_set_def assms TypedEqui.atrue_def atrue_twice_equal mem_Collect_eq subsetI)
 
 
 (*
-| "translate \<Gamma> F ({P1} C1 {Q1} || {P2} C2 {Q2}) =
+| "translate \<Gamma> ({P1} C1 {Q1} || {P2} C2 {Q2}) =
   ((Exhale (P1 \<otimes> P2);; ConcreteSemantics.havoc_list (wrL C1 @ wrL C2);; Inhale (Q1 \<otimes> Q2)),
-  let r1 = translate \<Gamma> F C1 in let r2 = translate \<Gamma> F C2 in
+  let r1 = translate \<Gamma> C1 in let r2 = translate \<Gamma> C2 in
   { (Inhale P1;; fst r1;; Exhale Q1), (Inhale P2;; fst r2;; Exhale Q2) } \<union> snd r1 \<union> snd r2)"
 *)
 
 
 lemma typed_self_framing_star:
-  assumes "TypedEqui.self_framing_typed \<Delta> A"
-      and "TypedEqui.self_framing_typed \<Delta> B"
-    shows "TypedEqui.self_framing_typed \<Delta> (A \<otimes> B)"
+  assumes "TypedEqui.self_framing_typed tcfe A"
+      and "TypedEqui.self_framing_typed tcfe B"
+    shows "TypedEqui.self_framing_typed tcfe (A \<otimes> B)"
 proof (rule TypedEqui.self_framing_typedI)
-  fix \<omega> assume asm0: "TypedEqui.typed \<Delta> \<omega>"
+  fix \<omega>
+  assume asm0: "typed tcfe \<omega>"
   show "(\<omega> \<in> A \<otimes> B) = (stabilize \<omega> \<in> A \<otimes> B)"
   proof
     assume "\<omega> \<in> A \<otimes> B"
@@ -646,7 +678,7 @@ proof (rule TypedEqui.self_framing_typedI)
       by (metis (no_types, opaque_lifting) asso2 decompose_stabilize_pure option.exhaust_sel)
     then have "stabilize b' = stabilize b"
       using plus_pure_stabilize_eq by blast
-    moreover have "TypedEqui.typed \<Delta> b'"
+    moreover have "TypedEqui.typed tcfe b'"
       by (smt (verit, ccfv_SIG) TypedEqui.typed_state_axioms \<open>Some (stabilize \<omega>) = a \<oplus> b\<close> \<open>Some b' = b \<oplus> |\<omega>|\<close> addition_bigger asm0 commutative decompose_stabilize_pure greater_def typed_state.typed_smaller)
     ultimately have "b' \<in> B"
       by (metis (no_types, lifting) TypedEqui.typed_smaller TypedEqui.typed_state_axioms \<open>Some b' = b \<oplus> |\<omega>|\<close> \<open>b \<in> B\<close> assms(2) commutative greater_equiv typed_state.self_framing_typed_def)
@@ -658,123 +690,125 @@ qed
 
 
 lemma self_framing_typed_star_atrue:
-  assumes "TypedEqui.self_framing_typed \<Delta> P"
-  shows "TypedEqui.self_framing_typed \<Delta> (P \<otimes> atrue \<Delta>)"
+  assumes "TypedEqui.self_framing_typed tcfe P"
+  shows "TypedEqui.self_framing_typed tcfe (P \<otimes> atrue tcfe)"
   by (simp add: assms typed_self_framing_star)
 
 lemma typed_assertion_star_atrue:
-  assumes "TypedEqui.typed_assertion \<Delta> P"
-  shows "TypedEqui.typed_assertion \<Delta> (P \<otimes> atrue \<Delta>)"
+  assumes "TypedEqui.typed_assertion tcfe P"
+  shows "TypedEqui.typed_assertion tcfe (P \<otimes> atrue tcfe)"
   by (simp add: TypedEqui.typed_star assms)
 
 
 
 
 lemma invariant_translate_parallel:
-  assumes "\<And>P Q. invariant_translate \<Gamma> F \<Delta> P C1 Q"
-      and "\<And>P Q. invariant_translate \<Gamma> F \<Delta> P C2 Q"
-      and "ConcreteSemantics.wf_abs_stmt \<Delta> (ConcreteSemantics.havoc_list (wrL C1 @ wrL C2))"
-      and "wf_stmt \<Gamma> F \<Delta> ({P1} C1 {Q1} || {P2} C2 {Q2})"
-      and "TypedEqui.wf_context \<Delta>"
-    shows "invariant_translate \<Gamma> F \<Delta> P ({P1} C1 {Q1} || {P2} C2 {Q2}) Q"
+  assumes "\<And>P Q. invariant_translate \<Gamma> P C1 Q"
+      and "\<And>P Q. invariant_translate \<Gamma> P C2 Q"
+      and "ConcreteSemantics.wf_abs_stmt tcfe (ConcreteSemantics.havoc_list (wrL C1 @ wrL C2))"
+      and "wf_stmt \<Gamma> F ({P1} C1 {Q1} || {P2} C2 {Q2})"
+      and "TypedEqui.wf_context tcfe"
+    shows "invariant_translate \<Gamma> P ({P1} C1 {Q1} || {P2} C2 {Q2}) Q"
 proof (rule invariant_translateI)
-  let ?P1 = "make_semantic_assertion \<Gamma> F P1"
-  let ?P2 = "make_semantic_assertion \<Gamma> F P2"
-  let ?Q1 = "make_semantic_assertion \<Gamma> F Q1"
-  let ?Q2 = "make_semantic_assertion \<Gamma> F Q2"
+  let ?P1 = "make_semantic_assertion \<Gamma> type_ctxt_front_end_syntactic P1"
+  let ?P2 = "make_semantic_assertion \<Gamma> type_ctxt_front_end_syntactic P2"
+  let ?Q1 = "make_semantic_assertion \<Gamma> type_ctxt_front_end_syntactic Q1"
+  let ?Q2 = "make_semantic_assertion \<Gamma> type_ctxt_front_end_syntactic Q2"
 
-  assume asm0: "proof_obligations_valid \<Delta> (snd (translate \<Gamma> F {P1} C1 {Q1} || {P2} C2 {Q2}))"
-    "ConcreteSemantics.SL_proof \<Delta> P (fst (translate \<Gamma> F {P1} C1 {Q1} || {P2} C2 {Q2})) Q"
-  then have r0: "proof_obligations_valid \<Delta> (snd (translate \<Gamma> F C1)) \<and> proof_obligations_valid \<Delta> (snd (translate \<Gamma> F C2))"
+  assume asm0: "proof_obligations_valid (snd (translate \<Gamma> {P1} C1 {Q1} || {P2} C2 {Q2}))"
+    "ConcreteSemantics.SL_proof tcfe P (fst (translate \<Gamma> {P1} C1 {Q1} || {P2} C2 {Q2})) Q"
+  then have r0: "proof_obligations_valid (snd (translate \<Gamma> C1)) \<and> proof_obligations_valid (snd (translate \<Gamma> C2))"
     using proof_obligations_valid_union
     unfolding translate.simps by (metis sndI)
-  moreover obtain B1 where B1_def: "ConcreteSemantics.SL_proof \<Delta> (atrue \<Delta>)
-    (Inhale (make_semantic_assertion \<Gamma> F P1);; fst (translate \<Gamma> F C1);; Exhale (make_semantic_assertion \<Gamma> F Q1)) B1"
+  moreover obtain B1 where B1_def: "ConcreteSemantics.SL_proof tcfe (atrue tcfe)
+    (Inhale (make_semantic_assertion \<Gamma> type_ctxt_front_end_syntactic P1);; fst (translate \<Gamma> C1);; Exhale (make_semantic_assertion \<Gamma> type_ctxt_front_end_syntactic Q1)) B1"
     using asm0 unfolding translate.simps proof_obligations_valid_def
     by (metis Un_iff insertCI snd_eqD)
-  moreover obtain B2 where B2_def: "ConcreteSemantics.SL_proof \<Delta> (atrue \<Delta>)
-  (Inhale (make_semantic_assertion \<Gamma> F P2);; fst (translate \<Gamma> F C2);; Exhale (make_semantic_assertion \<Gamma> F Q2)) B2"
+  moreover obtain B2 where B2_def: "ConcreteSemantics.SL_proof tcfe (atrue tcfe)
+  (Inhale (make_semantic_assertion \<Gamma> type_ctxt_front_end_syntactic P2);; fst (translate \<Gamma> C2);; Exhale (make_semantic_assertion \<Gamma> type_ctxt_front_end_syntactic Q2)) B2"
     using asm0 unfolding translate.simps proof_obligations_valid_def
     by (metis Un_iff insertCI snd_eqD)
-  moreover have main: "ConcreteSemantics.SL_proof \<Delta> P (Exhale (make_semantic_assertion \<Gamma> F P1 \<otimes> make_semantic_assertion \<Gamma> F P2);;
+  moreover have main: "ConcreteSemantics.SL_proof tcfe P (Exhale (make_semantic_assertion \<Gamma> type_ctxt_front_end_syntactic P1 \<otimes> make_semantic_assertion \<Gamma> type_ctxt_front_end_syntactic P2);;
   ConcreteSemantics.havoc_list (wrL C1 @ wrL C2);;
-  Inhale (make_semantic_assertion \<Gamma> F Q1 \<otimes> make_semantic_assertion \<Gamma> F Q2)) Q"
+  Inhale (make_semantic_assertion \<Gamma> type_ctxt_front_end_syntactic Q1 \<otimes> make_semantic_assertion \<Gamma> type_ctxt_front_end_syntactic Q2)) Q"
     using asm0 by simp
   then obtain R0 R1 where R_defs:
-    "ConcreteSemantics.SL_proof \<Delta> P (abs_stmt.Exhale (make_semantic_assertion \<Gamma> F P1 \<otimes> make_semantic_assertion \<Gamma> F P2)) R0"
-    "ConcreteSemantics.SL_proof \<Delta> R0 (ConcreteSemantics.havoc_list (wrL C1 @ wrL C2)) R1"
-    "ConcreteSemantics.SL_proof \<Delta> R1 (abs_stmt.Inhale (make_semantic_assertion \<Gamma> F Q1 \<otimes> make_semantic_assertion \<Gamma> F Q2)) Q"
+    "ConcreteSemantics.SL_proof tcfe P (abs_stmt.Exhale (make_semantic_assertion \<Gamma> type_ctxt_front_end_syntactic P1 \<otimes> make_semantic_assertion \<Gamma> type_ctxt_front_end_syntactic P2)) R0"
+    "ConcreteSemantics.SL_proof tcfe R0 (ConcreteSemantics.havoc_list (wrL C1 @ wrL C2)) R1"
+    "ConcreteSemantics.SL_proof tcfe R1 (abs_stmt.Inhale (make_semantic_assertion \<Gamma> type_ctxt_front_end_syntactic Q1 \<otimes> make_semantic_assertion \<Gamma> type_ctxt_front_end_syntactic Q2)) Q"
     by (meson ConcreteSemantics.SL_proof_Seq_elim)
   then have P_Q_R_rels:
-    "entails P (R0 \<otimes> (make_semantic_assertion \<Gamma> F P1 \<otimes> make_semantic_assertion \<Gamma> F P2))
-  \<and> Q = R1 \<otimes> (make_semantic_assertion \<Gamma> F Q1 \<otimes> make_semantic_assertion \<Gamma> F Q2)" by auto
-  moreover have "entails R0 R1 \<and> fvA \<Delta> R1 \<subseteq> fvA \<Delta> R0 - (set (wrL C1 @ wrL C2))"
-    using ConcreteSemantics.SL_proof_Havoc_list_elim R_defs(2) assms(3) assms(5) by blast
+    "entails P (R0 \<otimes> (make_semantic_assertion \<Gamma> type_ctxt_front_end_syntactic P1 \<otimes> make_semantic_assertion \<Gamma> type_ctxt_front_end_syntactic P2))
+  \<and> Q = R1 \<otimes> (make_semantic_assertion \<Gamma> type_ctxt_front_end_syntactic Q1 \<otimes> make_semantic_assertion \<Gamma> type_ctxt_front_end_syntactic Q2)" by auto
+  moreover have r: "ConcreteSemantics.self_framing_and_typed tcfe R0 \<and>
+    ConcreteSemantics.self_framing_and_typed tcfe R1 \<and> entails R0 R1 \<and> fvA tcfe R1 \<subseteq> fvA tcfe R0 - set (wrL C1 @ wrL C2)"
+    using ConcreteSemantics.SL_proof_Havoc_list_elim[OF R_defs(2) assms(3) assms(5)] by blast
+
 (* R1 is the frame! *)
 
-  show "\<Delta> \<turnstile>CSL [P \<otimes> atrue \<Delta>] {P1} C1 {Q1} || {P2} C2 {Q2} [Q \<otimes> atrue \<Delta>]"
+  show "tcfe \<turnstile>CSL [P \<otimes> atrue tcfe] {P1} C1 {Q1} || {P2} C2 {Q2} [Q \<otimes> atrue tcfe]"
   proof (rule RuleCons)
-    show "\<Delta> \<turnstile>CSL [((?P1 \<otimes> atrue \<Delta>) \<otimes> (?P2 \<otimes> atrue \<Delta>)) \<otimes> R1] {P1} C1 {Q1} || {P2} C2 {Q2} [((?Q1 \<otimes> atrue \<Delta>) \<otimes> (?Q2 \<otimes> atrue \<Delta>)) \<otimes> R1]"
+    show "tcfe \<turnstile>CSL [((?P1 \<otimes> atrue tcfe) \<otimes> (?P2 \<otimes> atrue tcfe)) \<otimes> R1] {P1} C1 {Q1} || {P2} C2 {Q2} [((?Q1 \<otimes> atrue tcfe) \<otimes> (?Q2 \<otimes> atrue tcfe)) \<otimes> R1]"
     proof (rule RuleFrame)
-      show "\<Delta> \<turnstile>CSL [?P1 \<otimes> atrue \<Delta> \<otimes> (?P2 \<otimes> atrue \<Delta>)] {P1} C1 {Q1} || {P2} C2 {Q2} [?Q1 \<otimes> atrue \<Delta> \<otimes> (?Q2 \<otimes> atrue \<Delta>)]"
+      show "tcfe \<turnstile>CSL [?P1 \<otimes> atrue tcfe \<otimes> (?P2 \<otimes> atrue tcfe)] {P1} C1 {Q1} || {P2} C2 {Q2} [?Q1 \<otimes> atrue tcfe \<otimes> (?Q2 \<otimes> atrue tcfe)]"
       proof (rule RulePar)
-        show "\<Delta> \<turnstile>CSL [?P1 \<otimes> atrue \<Delta>] C1 [?Q1 \<otimes> atrue \<Delta>]"
+        show "tcfe \<turnstile>CSL [?P1 \<otimes> atrue tcfe] C1 [?Q1 \<otimes> atrue tcfe]"
         proof (rule RuleCons)
-          show "\<Delta> \<turnstile>CSL [atrue \<Delta> \<otimes> ?P1 \<otimes> atrue \<Delta>] C1 [B1 \<otimes> ?Q1 \<otimes> atrue \<Delta>]"
+          show "tcfe \<turnstile>CSL [atrue tcfe \<otimes> ?P1 \<otimes> atrue tcfe] C1 [B1 \<otimes> ?Q1 \<otimes> atrue tcfe]"
             using invariant_translate_inhale_exhale_get_proof[OF assms(1) B1_def]
             using r0 by blast
-          show "B1 \<otimes> ?Q1 \<otimes> atrue \<Delta> \<subseteq> ?Q1 \<otimes> atrue \<Delta>"
+          show "B1 \<otimes> ?Q1 \<otimes> atrue tcfe \<subseteq> ?Q1 \<otimes> atrue tcfe"
             using B1_def drop_conjunct_entails by blast
-          show "?P1 \<otimes> atrue \<Delta> \<subseteq> atrue \<Delta> \<otimes> ?P1 \<otimes> atrue \<Delta>"
-            using add_set_asso assms(4) conjunct_with_true_entails typed_assertion_star_atrue wf_stmt.simps(3) by blast
+          show "?P1 \<otimes> atrue tcfe \<subseteq> atrue tcfe \<otimes> ?P1 \<otimes> atrue tcfe"
+            by (metis (no_types, lifting) add_set_asso add_set_commm atrue_twice_equal order_refl)
         qed
-        show "\<Delta> \<turnstile>CSL [?P2 \<otimes> atrue \<Delta>] C2 [?Q2 \<otimes> atrue \<Delta>]"
+        show "tcfe \<turnstile>CSL [?P2 \<otimes> atrue tcfe] C2 [?Q2 \<otimes> atrue tcfe]"
         proof (rule RuleCons)
-          show "\<Delta> \<turnstile>CSL [atrue \<Delta> \<otimes> ?P2 \<otimes> atrue \<Delta>] C2 [B2 \<otimes> ?Q2 \<otimes> atrue \<Delta>]"
+          show "tcfe \<turnstile>CSL [atrue tcfe \<otimes> ?P2 \<otimes> atrue tcfe] C2 [B2 \<otimes> ?Q2 \<otimes> atrue tcfe]"
             using invariant_translate_inhale_exhale_get_proof[OF assms(2) B2_def]
             using r0 by blast
-          show "B2 \<otimes> ?Q2 \<otimes> atrue \<Delta> \<subseteq> ?Q2 \<otimes> atrue \<Delta>"
+          show "B2 \<otimes> ?Q2 \<otimes> atrue tcfe \<subseteq> ?Q2 \<otimes> atrue tcfe"
             using B2_def drop_conjunct_entails by blast
-          show "?P2 \<otimes> atrue \<Delta> \<subseteq> atrue \<Delta> \<otimes> ?P2 \<otimes> atrue \<Delta>"
+          show "?P2 \<otimes> atrue tcfe \<subseteq> atrue tcfe \<otimes> ?P2 \<otimes> atrue tcfe"
             using add_set_asso add_set_left_comm atrue_twice_equal
             by (metis (no_types, opaque_lifting) order_refl)
         qed
-        show "disjoint (fvC C1 \<union> fvA \<Delta> (?Q1 \<otimes> atrue \<Delta>)) (wrC C2)"
+        show "disjoint (fvC C1 \<union> fvA tcfe (?Q1 \<otimes> atrue tcfe)) (wrC C2)"
           using assms(4) by auto
-        show "disjoint (fvC C2 \<union> fvA \<Delta> (?Q2 \<otimes> atrue \<Delta>)) (wrC C1)"
+        show "disjoint (fvC C2 \<union> fvA tcfe (?Q2 \<otimes> atrue tcfe)) (wrC C1)"
           using assms(4) by auto
-        show "TypedEqui.self_framing_typed \<Delta> (?P1 \<otimes> atrue \<Delta>)"
-          using assms(4) self_framing_typed_star_atrue wf_stmt.simps(3) by blast
-        show "TypedEqui.self_framing_typed \<Delta> (?P2 \<otimes> atrue \<Delta>)"
+        show "TypedEqui.self_framing_typed tcfe (?P1 \<otimes> atrue tcfe)"
+          using assms(4) typed_self_framing_star by fastforce
+        show "TypedEqui.self_framing_typed tcfe (?P2 \<otimes> atrue tcfe)"
           using assms(4) self_framing_typed_star_atrue by auto
-        show "TypedEqui.typed_assertion \<Delta> (?P1 \<otimes> atrue \<Delta>)"
+        show "TypedEqui.typed_assertion tcfe (?P1 \<otimes> atrue tcfe)"
           using assms(4) typed_assertion_star_atrue by auto
-        show "TypedEqui.typed_assertion \<Delta> (?P2 \<otimes> atrue \<Delta>)"
+        show "TypedEqui.typed_assertion tcfe (?P2 \<otimes> atrue tcfe)"
           using assms(4) typed_assertion_star_atrue by auto
       qed
-      show "disjoint (fvA \<Delta> R1) (wrC {P1} C1 {Q1} || {P2} C2 {Q2})"
-        by (metis (mono_tags, opaque_lifting) Diff_subset_conv Orderings.order_eq_iff \<open>entails R0 R1 \<and> fvA \<Delta> R1 \<subseteq> fvA \<Delta> R0 - set (wrL C1 @ wrL C2)\<close> bot.extremum disjoint_minus disjoint_simps(2) disjoint_simps(3) sup.order_iff wrC.simps(7) wrC.simps(8) wrL.simps(7) wrL_wrC_same)
-      show "TypedEqui.self_framing_typed \<Delta> (?P1 \<otimes> atrue \<Delta> \<otimes> (?P2 \<otimes> atrue \<Delta>))"
+      show "disjoint (fvA tcfe R1) (wrC {P1} C1 {Q1} || {P2} C2 {Q2})"
+        by (metis (mono_tags, opaque_lifting) Diff_subset_conv Orderings.order_eq_iff r bot.extremum disjoint_minus disjoint_simps(2) disjoint_simps(3) sup.order_iff wrC.simps(7) wrC.simps(8) wrL.simps(7) wrL_wrC_same)
+      show "TypedEqui.self_framing_typed tcfe (?P1 \<otimes> atrue tcfe \<otimes> (?P2 \<otimes> atrue tcfe))"
         by (meson assms(4) self_framing_typed_star_atrue typed_self_framing_star wf_stmt.simps(3))
-      show "TypedEqui.typed_assertion \<Delta> (?P1 \<otimes> atrue \<Delta> \<otimes> (?P2 \<otimes> atrue \<Delta>))"
-        using TypedEqui.typed_star assms(4) typed_assertion_star_atrue wf_stmt.simps(3) by blast
-      show "TypedEqui.self_framing_typed \<Delta> R1"
+      show "TypedEqui.typed_assertion tcfe (?P1 \<otimes> atrue tcfe \<otimes> (?P2 \<otimes> atrue tcfe))"
+        using TypedEqui.typed_star assms(4) typed_assertion_star_atrue by auto
+      show "TypedEqui.self_framing_typed tcfe R1"
         using R_defs(3) by blast
-      show "TypedEqui.typed_assertion \<Delta> R1"
+      show "TypedEqui.typed_assertion tcfe R1"
         using R_defs(3) by force
     qed
-    show "P \<otimes> atrue \<Delta> \<subseteq> ?P1 \<otimes> atrue \<Delta> \<otimes> (?P2 \<otimes> atrue \<Delta>) \<otimes> R1"
+    show "P \<otimes> atrue tcfe \<subseteq> ?P1 \<otimes> atrue tcfe \<otimes> (?P2 \<otimes> atrue tcfe) \<otimes> R1"
     proof -
-      have "P \<otimes> atrue \<Delta> \<subseteq> (R0 \<otimes> (?P1 \<otimes> ?P2)) \<otimes> atrue \<Delta>"
+      have "P \<otimes> atrue tcfe \<subseteq> (R0 \<otimes> (?P1 \<otimes> ?P2)) \<otimes> atrue tcfe"
         by (metis P_Q_R_rels add_set_mono atrue_twice_equal atrue_twice_same entails_def)
-      also have "... \<subseteq> R1 \<otimes> ((?P1 \<otimes> ?P2) \<otimes> atrue \<Delta>)"
-        using \<open>entails R0 R1 \<and> fvA \<Delta> R1 \<subseteq> fvA \<Delta> R0 - set (wrL C1 @ wrL C2)\<close> add_set_asso add_set_mono entails_def by blast
-      also have "... \<subseteq> ?P1 \<otimes> atrue \<Delta> \<otimes> (?P2 \<otimes> atrue \<Delta>) \<otimes> R1"
+      also have "... \<subseteq> R1 \<otimes> ((?P1 \<otimes> ?P2) \<otimes> atrue tcfe)"
+        using r add_set_asso add_set_mono entails_def by blast
+      also have "... \<subseteq> ?P1 \<otimes> atrue tcfe \<otimes> (?P2 \<otimes> atrue tcfe) \<otimes> R1"
         using add_set_commm add_set_left_comm atrue_twice_equal
         by (smt (verit, del_insts) dual_order.refl)
       finally show ?thesis by simp
     qed
-    show "?Q1 \<otimes> atrue \<Delta> \<otimes> (?Q2 \<otimes> atrue \<Delta>) \<otimes> R1 \<subseteq> Q \<otimes> atrue \<Delta>"
+    show "?Q1 \<otimes> atrue tcfe \<otimes> (?Q2 \<otimes> atrue tcfe) \<otimes> R1 \<subseteq> Q \<otimes> atrue tcfe"
       by (metis (no_types, lifting) Orderings.order_eq_iff P_Q_R_rels add_set_asso add_set_commm atrue_twice_equal)
   qed
 qed
@@ -782,9 +816,9 @@ qed
 (*
 Maybe prove? Need to prove that assertions are wf...
 lemma translation_wf:
-  assumes "wf_stmt \<Gamma> F \<Delta> C"
-      and "well_typed_cmd \<Delta> C"
-    shows "ConcreteSemantics.wf_abs_stmt \<Delta> (fst (translate \<Gamma> F C))"
+  assumes "wf_stmt \<Gamma> F C"
+      and "well_typed_cmd tcfe C"
+    shows "ConcreteSemantics.wf_abs_stmt tcfe (fst (translate \<Gamma> C))"
   using assms
 proof (induct C)
   case (Cseq C1 C2)
@@ -796,66 +830,66 @@ qed (simp_all)
 *)
 
 lemma invariant_translate_if:
-  assumes "\<And>P Q. invariant_translate \<Gamma> F \<Delta> P C1 Q"
-      and "\<And>P Q. invariant_translate \<Gamma> F \<Delta> P C2 Q"
-    shows "invariant_translate \<Gamma> F \<Delta> P (Cif b C1 C2) Q"
+  assumes "\<And>P Q. invariant_translate \<Gamma> P C1 Q"
+      and "\<And>P Q. invariant_translate \<Gamma> P C2 Q"
+    shows "invariant_translate \<Gamma> P (Cif b C1 C2) Q"
 proof (rule invariant_translateI)
-  assume asm0: "proof_obligations_valid \<Delta> (snd (translate \<Gamma> F (Cif b C1 C2)))"
-    "ConcreteSemantics.SL_proof \<Delta> P (fst (translate \<Gamma> F (Cif b C1 C2))) Q"
+  assume asm0: "proof_obligations_valid (snd (translate \<Gamma> (Cif b C1 C2)))"
+    "ConcreteSemantics.SL_proof tcfe P (fst (translate \<Gamma> (Cif b C1 C2))) Q"
 
-  show "\<Delta> \<turnstile>CSL [P \<otimes> atrue \<Delta>] Cif b C1 C2 [Q \<otimes> atrue \<Delta>]"
+  show "tcfe \<turnstile>CSL [P \<otimes> atrue tcfe] Cif b C1 C2 [Q \<otimes> atrue tcfe]"
   proof (rule ConcreteSemantics.SL_proof_If_elim)
-    show "ConcreteSemantics.SL_proof \<Delta> P (abs_stmt.If (semantify_bexp b) (fst (translate \<Gamma> F C1)) (fst (translate \<Gamma> F C2))) Q"
+    show "ConcreteSemantics.SL_proof tcfe P (abs_stmt.If (semantify_bexp b) (fst (translate \<Gamma> C1)) (fst (translate \<Gamma> C2))) Q"
       by (metis asm0(2) fst_eqD translate.simps(8))
     fix B1 B2 assume asm1: "Q = B1 \<union> B2" "framed_by_exp P (semantify_bexp b)"
-       "ConcreteSemantics.SL_proof \<Delta> (P \<otimes> ConcreteSemantics.pure_typed \<Delta> (semantify_bexp b)) (fst (translate \<Gamma> F C1)) B1"
-       "ConcreteSemantics.SL_proof \<Delta> (P \<otimes> ConcreteSemantics.pure_typed \<Delta> (negate (semantify_bexp b))) (fst (translate \<Gamma> F C2)) B2"
-       "TypedEqui.self_framing_typed \<Delta> P" "TypedEqui.typed_assertion \<Delta> P"
-    show "\<Delta> \<turnstile>CSL [P \<otimes> atrue \<Delta>] Cif b C1 C2 [Q \<otimes> atrue \<Delta>]"
+       "ConcreteSemantics.SL_proof tcfe (P \<otimes> ConcreteSemantics.pure_typed tcfe (semantify_bexp b)) (fst (translate \<Gamma> C1)) B1"
+       "ConcreteSemantics.SL_proof tcfe (P \<otimes> ConcreteSemantics.pure_typed tcfe (negate (semantify_bexp b))) (fst (translate \<Gamma> C2)) B2"
+       "TypedEqui.self_framing_typed tcfe P" "TypedEqui.typed_assertion tcfe P"
+    show "tcfe \<turnstile>CSL [P \<otimes> atrue tcfe] Cif b C1 C2 [Q \<otimes> atrue tcfe]"
     proof (rule RuleIf)
-      show "\<Delta> \<turnstile>CSL [(P \<otimes> atrue \<Delta>) \<inter> assertify_bexp b] C1 [Q \<otimes> atrue \<Delta>]"
+      show "tcfe \<turnstile>CSL [(P \<otimes> atrue tcfe) \<inter> assertify_bexp b] C1 [Q \<otimes> atrue tcfe]"
       proof (rule RuleCons)
-        show "\<Delta> \<turnstile>CSL [(P \<otimes> ConcreteSemantics.pure_typed \<Delta> (semantify_bexp b)) \<otimes> atrue \<Delta>] C1 [B1 \<otimes> atrue \<Delta>]"
+        show "tcfe \<turnstile>CSL [(P \<otimes> ConcreteSemantics.pure_typed tcfe (semantify_bexp b)) \<otimes> atrue tcfe] C1 [B1 \<otimes> atrue tcfe]"
           by (metis asm0(1) asm1(3) assms(1) invariant_translateE proof_obligations_valid_union snd_conv translate.simps(8))
-        show "B1 \<otimes> atrue \<Delta> \<subseteq> Q \<otimes> atrue \<Delta>"
+        show "B1 \<otimes> atrue tcfe \<subseteq> Q \<otimes> atrue tcfe"
           by (simp add: add_set_mono asm1(1))
-        show "(P \<otimes> atrue \<Delta>) \<inter> assertify_bexp b \<subseteq> (P \<otimes> ConcreteSemantics.pure_typed \<Delta> (semantify_bexp b)) \<otimes> atrue \<Delta>"
+        show "(P \<otimes> atrue tcfe) \<inter> assertify_bexp b \<subseteq> (P \<otimes> ConcreteSemantics.pure_typed tcfe (semantify_bexp b)) \<otimes> atrue tcfe"
         proof
-          fix \<omega> assume "\<omega> \<in> (P \<otimes> atrue \<Delta>) \<inter> assertify_bexp b"
+          fix \<omega> assume "\<omega> \<in> (P \<otimes> atrue tcfe) \<inter> assertify_bexp b"
           then obtain p r where "Some \<omega> = p \<oplus> r" "p \<in> P" "bdenot b (get_store \<omega>)"
-            using in_set_sum[of \<omega> P "atrue \<Delta>"] assertify_bexp_def
+            using in_set_sum[of \<omega> P "atrue tcfe"] assertify_bexp_def
             by (smt (verit) Int_iff commutative greater_equiv mem_Collect_eq)
-          then have "|p| \<in> ConcreteSemantics.pure_typed \<Delta> (semantify_bexp b)"
+          then have "|p| \<in> ConcreteSemantics.pure_typed tcfe (semantify_bexp b)"
             unfolding ConcreteSemantics.pure_typed_def semantify_bexp_def
             by (smt (verit, ccfv_SIG) ConcreteSemantics.get_store_Ag_simplifies TypedEqui.typed_assertionE TypedEqui.typed_core asm1(6) full_add_charact(1) full_core_def max_projection_prop_pure_core mem_Collect_eq mpp_prop)
-          then have "p \<in> P \<otimes> ConcreteSemantics.pure_typed \<Delta> (semantify_bexp b)"
+          then have "p \<in> P \<otimes> ConcreteSemantics.pure_typed tcfe (semantify_bexp b)"
             using \<open>p \<in> P\<close> core_is_smaller x_elem_set_product by blast
-          then show "\<omega> \<in> (P \<otimes> ConcreteSemantics.pure_typed \<Delta> (semantify_bexp b)) \<otimes> atrue \<Delta>"
-            using TypedEqui.typed_state_axioms \<open>Some \<omega> = p \<oplus> r\<close> \<open>\<omega> \<in> (P \<otimes> atrue \<Delta>) \<inter> assertify_bexp b\<close> asm1(6) greater_def in_times_atrue typed_assertion_star_atrue typed_state.typed_assertionE by blast
+          then show "\<omega> \<in> (P \<otimes> ConcreteSemantics.pure_typed tcfe (semantify_bexp b)) \<otimes> atrue tcfe"
+            using TypedEqui.typed_state_axioms \<open>Some \<omega> = p \<oplus> r\<close> \<open>\<omega> \<in> (P \<otimes> atrue tcfe) \<inter> assertify_bexp b\<close> asm1(6) greater_def in_times_atrue typed_assertion_star_atrue typed_state.typed_assertionE by blast
         qed
       qed
 
-      show "\<Delta> \<turnstile>CSL [(P \<otimes> atrue \<Delta>) \<inter> assertify_bexp (Bnot b)] C2 [Q \<otimes> atrue \<Delta>]"
+      show "tcfe \<turnstile>CSL [(P \<otimes> atrue tcfe) \<inter> assertify_bexp (Bnot b)] C2 [Q \<otimes> atrue tcfe]"
       proof (rule RuleCons)
-        show "\<Delta> \<turnstile>CSL [(P \<otimes> ConcreteSemantics.pure_typed \<Delta> (negate (semantify_bexp b))) \<otimes> atrue \<Delta>] C2 [B2 \<otimes> atrue \<Delta>]"
+        show "tcfe \<turnstile>CSL [(P \<otimes> ConcreteSemantics.pure_typed tcfe (negate (semantify_bexp b))) \<otimes> atrue tcfe] C2 [B2 \<otimes> atrue tcfe]"
           by (metis asm0(1) asm1(4) assms(2) invariant_translateE proof_obligations_valid_union snd_conv translate.simps(8))
-        show "B2 \<otimes> atrue \<Delta> \<subseteq> Q \<otimes> atrue \<Delta>"
+        show "B2 \<otimes> atrue tcfe \<subseteq> Q \<otimes> atrue tcfe"
           by (simp add: add_set_mono asm1(1))
-        show "(P \<otimes> atrue \<Delta>) \<inter> assertify_bexp (Bnot b) \<subseteq> P \<otimes> ConcreteSemantics.pure_typed \<Delta> (negate (semantify_bexp b)) \<otimes> atrue \<Delta>"
+        show "(P \<otimes> atrue tcfe) \<inter> assertify_bexp (Bnot b) \<subseteq> P \<otimes> ConcreteSemantics.pure_typed tcfe (negate (semantify_bexp b)) \<otimes> atrue tcfe"
         proof
-          fix \<omega> assume "\<omega> \<in> (P \<otimes> atrue \<Delta>) \<inter> assertify_bexp (Bnot b)"
+          fix \<omega> assume "\<omega> \<in> (P \<otimes> atrue tcfe) \<inter> assertify_bexp (Bnot b)"
           then obtain p r where "Some \<omega> = p \<oplus> r" "p \<in> P" "bdenot (Bnot b) (get_store \<omega>)"
-            using in_set_sum[of \<omega> P "atrue \<Delta>"] assertify_bexp_def
+            using in_set_sum[of \<omega> P "atrue tcfe"] assertify_bexp_def
             by (smt (verit) Int_iff commutative greater_equiv mem_Collect_eq)
           then have "\<not> bdenot b (get_store |p| )"
             by (simp add: core_charact(1) full_add_charact(1))
-          then have "|p| \<in> ConcreteSemantics.pure_typed \<Delta> (negate (semantify_bexp b))"
+          then have "|p| \<in> ConcreteSemantics.pure_typed tcfe (negate (semantify_bexp b))"
             unfolding ConcreteSemantics.pure_typed_def semantify_bexp_def negate_def
             by (smt (verit, del_insts) CollectD CollectI TypedEqui.typed_assertionE TypedEqui.typed_core \<open>p \<in> P\<close> asm1(2) asm1(6) core_charact(1) core_in_emp_core emp_core_def framed_by_exp_def option.collapse semantify_bexp_def)
-          then have "p \<in> P \<otimes> ConcreteSemantics.pure_typed \<Delta> (negate (semantify_bexp b))"
+          then have "p \<in> P \<otimes> ConcreteSemantics.pure_typed tcfe (negate (semantify_bexp b))"
             using \<open>p \<in> P\<close> core_is_smaller x_elem_set_product by blast
-          then show "\<omega> \<in> (P \<otimes> ConcreteSemantics.pure_typed \<Delta> (negate (semantify_bexp b))) \<otimes> atrue \<Delta>"
-            by (meson TypedEqui.typed_intersection TypedEqui.typed_state_axioms \<open>Some \<omega> = p \<oplus> r\<close> \<open>\<omega> \<in> (P \<otimes> atrue \<Delta>) \<inter> assertify_bexp (Bnot b)\<close> asm1(6) atrue_self_framing_and_typed(1) greater_def in_times_atrue typed_state.typed_assertionE typed_state.typed_star)
+          then show "\<omega> \<in> (P \<otimes> ConcreteSemantics.pure_typed tcfe (negate (semantify_bexp b))) \<otimes> atrue tcfe"
+            by (meson TypedEqui.typed_intersection TypedEqui.typed_state_axioms \<open>Some \<omega> = p \<oplus> r\<close> \<open>\<omega> \<in> (P \<otimes> atrue tcfe) \<inter> assertify_bexp (Bnot b)\<close> asm1(6) atrue_self_framing_and_typed(1) greater_def in_times_atrue typed_state.typed_assertionE typed_state.typed_star)
         qed
       qed
     qed
@@ -876,72 +910,72 @@ qed
 
 
 lemma invariant_translate_while:
-  assumes "\<And>P Q. invariant_translate \<Gamma> F \<Delta> P C Q"
-      and "ConcreteSemantics.wf_abs_stmt \<Delta> (ConcreteSemantics.havoc_list (wrL C))"
-      and "wf_stmt \<Gamma> F \<Delta> (Cwhile b I C)"
-      and "TypedEqui.wf_context \<Delta>"
-    shows "invariant_translate \<Gamma> F \<Delta> P (Cwhile b I C) Q"
+  assumes "\<And>P Q. invariant_translate \<Gamma> P C Q"
+      and "ConcreteSemantics.wf_abs_stmt tcfe (ConcreteSemantics.havoc_list (wrL C))"
+      and "wf_stmt \<Gamma> F (Cwhile b I C)"
+      and "TypedEqui.wf_context tcfe"
+    shows "invariant_translate \<Gamma> P (Cwhile b I C) Q"
 proof (rule invariant_translateI)
-  let ?I = "make_semantic_assertion \<Gamma> F I"
-  assume asm0: "proof_obligations_valid \<Delta> (snd (translate \<Gamma> F (Cwhile b I C)))"
-    "ConcreteSemantics.SL_proof \<Delta> P (fst (translate \<Gamma> F (Cwhile b I C))) Q"
-  then have r1: "proof_obligations_valid \<Delta> (snd (translate \<Gamma> F C))"
+  let ?I = "make_semantic_assertion \<Gamma> type_ctxt_front_end_syntactic I"
+  assume asm0: "proof_obligations_valid (snd (translate \<Gamma> (Cwhile b I C)))"
+    "ConcreteSemantics.SL_proof tcfe P (fst (translate \<Gamma> (Cwhile b I C))) Q"
+  then have r1: "proof_obligations_valid (snd (translate \<Gamma> C))"
     using proof_obligations_valid_union by fastforce
-  moreover obtain B where B_def: "ConcreteSemantics.SL_proof \<Delta> (atrue \<Delta>) (Inhale (?I \<inter> assertify_bexp b);; fst (translate \<Gamma> F C);; Exhale ?I) B"
+  moreover obtain B where B_def: "ConcreteSemantics.SL_proof tcfe (atrue tcfe) (Inhale (?I \<inter> assertify_bexp b);; fst (translate \<Gamma> C);; Exhale ?I) B"
     by (metis (no_types, lifting) asm0(1) insertCI proof_obligations_valid_def proof_obligations_valid_union snd_eqD translate.simps(10))
   moreover obtain R0 R1 where R_defs: "entails P (R0 \<otimes> ?I)" "Q = R1 \<otimes> (?I \<inter> assertify_bexp (Bnot b))"
-    "ConcreteSemantics.SL_proof \<Delta> R0 (ConcreteSemantics.havoc_list (wrL C)) R1"
+    "ConcreteSemantics.SL_proof tcfe R0 (ConcreteSemantics.havoc_list (wrL C)) R1"
     using asm0(2) by auto
-  moreover have "entails R0 R1 \<and> fvA \<Delta> R1 \<subseteq> fvA \<Delta> R0 - (set (wrL C))"
+  moreover have "entails R0 R1 \<and> fvA tcfe R1 \<subseteq> fvA tcfe R0 - (set (wrL C))"
     using ConcreteSemantics.SL_proof_Havoc_list_elim assms(2) calculation(5) assms(4) by blast
 
   (* R1 is the frame *)
 
-  show "\<Delta> \<turnstile>CSL [P \<otimes> atrue \<Delta>] Cwhile b I C [Q \<otimes> atrue \<Delta>]"
+  show "tcfe \<turnstile>CSL [P \<otimes> atrue tcfe] Cwhile b I C [Q \<otimes> atrue tcfe]"
   proof (rule RuleCons)
-    show "\<Delta> \<turnstile>CSL [(?I \<otimes> atrue \<Delta>) \<otimes> R1] Cwhile b I C [((?I \<otimes> atrue \<Delta>) \<inter> (assertify_bexp (Bnot b))) \<otimes> R1]"
+    show "tcfe \<turnstile>CSL [(?I \<otimes> atrue tcfe) \<otimes> R1] Cwhile b I C [((?I \<otimes> atrue tcfe) \<inter> (assertify_bexp (Bnot b))) \<otimes> R1]"
     proof (rule RuleFrame)
-      show "\<Delta> \<turnstile>CSL [?I \<otimes> atrue \<Delta>] Cwhile b I C [(?I \<otimes> atrue \<Delta>) \<inter> assertify_bexp (Bnot b)]"
+      show "tcfe \<turnstile>CSL [?I \<otimes> atrue tcfe] Cwhile b I C [(?I \<otimes> atrue tcfe) \<inter> assertify_bexp (Bnot b)]"
       proof (rule RuleWhile)
-        show "\<Delta> \<turnstile>CSL [(?I \<otimes> atrue \<Delta>) \<inter> assertify_bexp b] C [?I \<otimes> atrue \<Delta>]"
+        show "tcfe \<turnstile>CSL [(?I \<otimes> atrue tcfe) \<inter> assertify_bexp b] C [?I \<otimes> atrue tcfe]"
         proof (rule RuleCons)
-          show "\<Delta> \<turnstile>CSL [atrue \<Delta> \<otimes> ?I \<inter> assertify_bexp b \<otimes> atrue \<Delta>] C [B \<otimes> ?I \<otimes> atrue \<Delta>]"
+          show "tcfe \<turnstile>CSL [atrue tcfe \<otimes> ?I \<inter> assertify_bexp b \<otimes> atrue tcfe] C [B \<otimes> ?I \<otimes> atrue tcfe]"
             using invariant_translate_inhale_exhale_get_proof[OF _ B_def]
             using assms(1) r1 by blast
-          show "B \<otimes> ?I \<otimes> atrue \<Delta> \<subseteq> ?I \<otimes> atrue \<Delta>"
+          show "B \<otimes> ?I \<otimes> atrue tcfe \<subseteq> ?I \<otimes> atrue tcfe"
             using B_def drop_conjunct_entails by blast
-          show "(?I \<otimes> atrue \<Delta>) \<inter> assertify_bexp b \<subseteq> atrue \<Delta> \<otimes> (?I \<inter> assertify_bexp b) \<otimes> atrue \<Delta>"
+          show "(?I \<otimes> atrue tcfe) \<inter> assertify_bexp b \<subseteq> atrue tcfe \<otimes> (?I \<inter> assertify_bexp b) \<otimes> atrue tcfe"
             by (metis (no_types, lifting) add_set_asso add_set_commm atrue_twice_equal intersect_and_star)
         qed
       qed
-      show "disjoint (fvA \<Delta> R1) (wrC (Cwhile b I C))"
-        using \<open>entails R0 R1 \<and> fvA \<Delta> R1 \<subseteq> fvA \<Delta> R0 - set (wrL C)\<close> disjoint_def wrL_wrC_same by fastforce
-      show "TypedEqui.self_framing_typed \<Delta> (?I \<otimes> atrue \<Delta>)"
+      show "disjoint (fvA tcfe R1) (wrC (Cwhile b I C))"
+        using \<open>entails R0 R1 \<and> fvA tcfe R1 \<subseteq> fvA tcfe R0 - set (wrL C)\<close> disjoint_def wrL_wrC_same by fastforce
+      show "TypedEqui.self_framing_typed tcfe (?I \<otimes> atrue tcfe)"
         using assms(3) self_framing_typed_star_atrue by auto
-      show "TypedEqui.self_framing_typed \<Delta> R1"
+      show "TypedEqui.self_framing_typed tcfe R1"
         using ConcreteSemantics.proofs_are_self_framing_and_typed assms(2) calculation(5) by blast
-      show "TypedEqui.typed_assertion \<Delta> (?I \<otimes> atrue \<Delta>)"
+      show "TypedEqui.typed_assertion tcfe (?I \<otimes> atrue tcfe)"
         using assms(3) typed_assertion_star_atrue by auto
-      show "TypedEqui.typed_assertion \<Delta> R1"
+      show "TypedEqui.typed_assertion tcfe R1"
         using ConcreteSemantics.proofs_are_self_framing_and_typed assms(2) calculation(5) by blast
     qed
     have "P \<subseteq> R1 \<otimes> ?I"
-      by (meson \<open>entails R0 R1 \<and> fvA \<Delta> R1 \<subseteq> fvA \<Delta> R0 - set (wrL C)\<close> add_set_mono calculation(3) entails_def equalityD1 subset_trans)
-    then show "P \<otimes> atrue \<Delta> \<subseteq> ?I \<otimes> atrue \<Delta> \<otimes> R1"
+      by (meson \<open>entails R0 R1 \<and> fvA tcfe R1 \<subseteq> fvA tcfe R0 - set (wrL C)\<close> add_set_mono calculation(3) entails_def equalityD1 subset_trans)
+    then show "P \<otimes> atrue tcfe \<subseteq> ?I \<otimes> atrue tcfe \<otimes> R1"
       by (smt (verit, best) add_set_asso add_set_commm add_set_mono atrue_twice_equal atrue_twice_same)
-    show "(?I \<otimes> atrue \<Delta>) \<inter> assertify_bexp (Bnot b) \<otimes> R1 \<subseteq> Q \<otimes> atrue \<Delta>"
+    show "(?I \<otimes> atrue tcfe) \<inter> assertify_bexp (Bnot b) \<otimes> R1 \<subseteq> Q \<otimes> atrue tcfe"
       by (smt (verit, del_insts) add_set_asso add_set_commm add_set_mono calculation(4) intersect_and_star subsetI)
   qed
 qed
 
 
 lemma invariant_translate_induct:
-  assumes "wf_stmt \<Gamma> F \<Delta> C"
-      and "well_typed_cmd \<Delta> C"
-      and "ConcreteSemantics.wf_abs_stmt \<Delta> (fst (translate \<Gamma> F C))"
-      and "\<And>Cv. Cv \<in> snd (translate \<Gamma> F C) \<Longrightarrow> ConcreteSemantics.wf_abs_stmt \<Delta> Cv"
-      and "TypedEqui.wf_context \<Delta>"
-    shows "invariant_translate \<Gamma> F \<Delta> P C Q"
+  assumes "wf_stmt \<Gamma> F C"
+      and "well_typed_cmd tcfe C"
+      and "ConcreteSemantics.wf_abs_stmt tcfe (fst (translate \<Gamma> C))"
+      and "\<And>Cv. Cv \<in> snd (translate \<Gamma> C) \<Longrightarrow> ConcreteSemantics.wf_abs_stmt tcfe Cv"
+      and "TypedEqui.wf_context tcfe"
+    shows "invariant_translate \<Gamma> P C Q"
   using assms
 proof (induct C arbitrary: P Q)
   case (Cseq C1 C2)
@@ -949,91 +983,91 @@ proof (induct C arbitrary: P Q)
     by (metis (no_types, lifting) ConcreteSemantics.wf_abs_stmt.simps(7) Un_iff fst_eqD invariant_translate_seq snd_conv translate.simps(7) well_typed_cmd_aux.simps(2) wf_stmt.simps(1))
 next
   case (Cpar P1 C1 Q1 P2 C2 Q2)
-  let ?P1 = "make_semantic_assertion \<Gamma> F P1"
-  let ?P2 = "make_semantic_assertion \<Gamma> F P2"
-  let ?Q1 = "make_semantic_assertion \<Gamma> F Q1"
-  let ?Q2 = "make_semantic_assertion \<Gamma> F Q2"
+  let ?P1 = "make_semantic_assertion \<Gamma> type_ctxt_front_end_syntactic P1"
+  let ?P2 = "make_semantic_assertion \<Gamma> type_ctxt_front_end_syntactic P2"
+  let ?Q1 = "make_semantic_assertion \<Gamma> type_ctxt_front_end_syntactic Q1"
+  let ?Q2 = "make_semantic_assertion \<Gamma> type_ctxt_front_end_syntactic Q2"
   show ?case
-  proof (rule invariant_translate_parallel[of _ _ \<Delta> C1 C2 P1 Q1 P2 Q2 P])
-    show "ConcreteSemantics.wf_abs_stmt \<Delta> (ConcreteSemantics.havoc_list (wrL C1 @ wrL C2))"
+  proof (rule invariant_translate_parallel)
+    show "ConcreteSemantics.wf_abs_stmt tcfe (ConcreteSemantics.havoc_list (wrL C1 @ wrL C2))"
       using Cpar.prems(3) by fastforce
-    show "wf_stmt \<Gamma> F \<Delta> {P1} C1 {Q1} || {P2} C2 {Q2}"
+    show "wf_stmt \<Gamma> F {P1} C1 {Q1} || {P2} C2 {Q2}"
       using Cpar.prems(1) by blast
     fix P Q
-    show "invariant_translate \<Gamma> F \<Delta> P C1 Q"
+    show "invariant_translate \<Gamma> P C1 Q"
     proof (rule Cpar(1))
-      have "ConcreteSemantics.wf_abs_stmt \<Delta> (Inhale ?P1;; fst (translate \<Gamma> F C1);; Exhale ?Q1)"
+      have "ConcreteSemantics.wf_abs_stmt tcfe (Inhale ?P1;; fst (translate \<Gamma> C1);; Exhale ?Q1)"
         by (metis Cpar.prems(4) Un_iff insertCI snd_eqD translate.simps(9))
-      then show "ConcreteSemantics.wf_abs_stmt \<Delta> (fst (translate \<Gamma> F C1))"
+      then show "ConcreteSemantics.wf_abs_stmt tcfe (fst (translate \<Gamma> C1))"
         by force
-      show "\<And>Cv. Cv \<in> snd (translate \<Gamma> F C1) \<Longrightarrow> ConcreteSemantics.wf_abs_stmt \<Delta> Cv"
+      show "\<And>Cv. Cv \<in> snd (translate \<Gamma> C1) \<Longrightarrow> ConcreteSemantics.wf_abs_stmt tcfe Cv"
         by (metis Cpar.prems(4) Un_iff snd_eqD translate.simps(9))
-      show "well_typed_cmd \<Delta> C1"
+      show "well_typed_cmd tcfe C1"
         using Cpar.prems(2) by auto
-      show "wf_stmt \<Gamma> F \<Delta> C1"
+      show "wf_stmt \<Gamma> F C1"
         using Cpar.prems(1) by auto
     qed (simp add: Cpar)
-    show "invariant_translate \<Gamma> F \<Delta> P C2 Q"
+    show "invariant_translate \<Gamma> P C2 Q"
     proof (rule Cpar(2))
-      have "ConcreteSemantics.wf_abs_stmt \<Delta> (Inhale ?P2;; fst (translate \<Gamma> F C2);; Exhale ?Q2)"
+      have "ConcreteSemantics.wf_abs_stmt tcfe (Inhale ?P2;; fst (translate \<Gamma> C2);; Exhale ?Q2)"
         by (metis Cpar.prems(4) Un_iff insertCI snd_eqD translate.simps(9))
-      then show "ConcreteSemantics.wf_abs_stmt \<Delta> (fst (translate \<Gamma> F C2))"
+      then show "ConcreteSemantics.wf_abs_stmt tcfe (fst (translate \<Gamma> C2))"
         by force
-      show "\<And>Cv. Cv \<in> snd (translate \<Gamma> F C2) \<Longrightarrow> ConcreteSemantics.wf_abs_stmt \<Delta> Cv"
+      show "\<And>Cv. Cv \<in> snd (translate \<Gamma> C2) \<Longrightarrow> ConcreteSemantics.wf_abs_stmt tcfe Cv"
         by (metis Cpar.prems(4) Un_iff snd_eqD translate.simps(9))
-      show "well_typed_cmd \<Delta> C2"
+      show "well_typed_cmd tcfe C2"
         using Cpar.prems(2) by auto
-      show "wf_stmt \<Gamma> F \<Delta> C2"
+      show "wf_stmt \<Gamma> F C2"
         using Cpar.prems(1) by auto
     qed (simp add: Cpar)
   qed (simp add: Cpar)
 next
   case (Cif b C1 C2)
   show ?case
-  proof (rule invariant_translate_if[of _ _ \<Delta> C1 C2 P b ])
+  proof (rule invariant_translate_if)
     fix P Q
-    show "invariant_translate \<Gamma> F \<Delta> P C1 Q"
+    show "invariant_translate \<Gamma> P C1 Q"
     proof (rule Cif(1))
-      show "wf_stmt \<Gamma> F \<Delta> C1"
+      show "wf_stmt \<Gamma> F C1"
         using Cif.prems(1) by auto
-      show "well_typed_cmd \<Delta> C1"
+      show "well_typed_cmd tcfe C1"
         using Cif.prems(2) by auto
-      show "ConcreteSemantics.wf_abs_stmt \<Delta> (fst (translate \<Gamma> F C1))"
+      show "ConcreteSemantics.wf_abs_stmt tcfe (fst (translate \<Gamma> C1))"
         using Cif.prems(3) by fastforce
-      show "\<And>Cv. Cv \<in> snd (translate \<Gamma> F C1) \<Longrightarrow> ConcreteSemantics.wf_abs_stmt \<Delta> Cv"
+      show "\<And>Cv. Cv \<in> snd (translate \<Gamma> C1) \<Longrightarrow> ConcreteSemantics.wf_abs_stmt tcfe Cv"
         by (metis Cif.prems(4) Un_iff snd_eqD translate.simps(8))
     qed (simp add: Cif)
-    show "invariant_translate \<Gamma> F \<Delta> P C2 Q"
+    show "invariant_translate \<Gamma> P C2 Q"
     proof (rule Cif(2))
-      show "wf_stmt \<Gamma> F \<Delta> C2"
+      show "wf_stmt \<Gamma> F C2"
         using Cif.prems(1) by auto
-      show "well_typed_cmd \<Delta> C2"
+      show "well_typed_cmd tcfe C2"
         using Cif.prems(2) by auto
-      show "ConcreteSemantics.wf_abs_stmt \<Delta> (fst (translate \<Gamma> F C2))"
+      show "ConcreteSemantics.wf_abs_stmt tcfe (fst (translate \<Gamma> C2))"
         using Cif.prems(3) by fastforce
-      show "\<And>Cv. Cv \<in> snd (translate \<Gamma> F C2) \<Longrightarrow> ConcreteSemantics.wf_abs_stmt \<Delta> Cv"
+      show "\<And>Cv. Cv \<in> snd (translate \<Gamma> C2) \<Longrightarrow> ConcreteSemantics.wf_abs_stmt tcfe Cv"
         by (metis Cif.prems(4) Un_iff snd_eqD translate.simps(8))
     qed (simp add: Cif)
   qed
 next
   case (Cwhile b I C)
-  let ?I = "make_semantic_assertion \<Gamma> F I"
+  let ?I = "make_semantic_assertion \<Gamma> type_ctxt_front_end_syntactic I"
   show ?case
   proof (rule invariant_translate_while)
-    show "ConcreteSemantics.wf_abs_stmt \<Delta> (ConcreteSemantics.havoc_list (wrL C))"
+    show "ConcreteSemantics.wf_abs_stmt tcfe (ConcreteSemantics.havoc_list (wrL C))"
       using Cwhile.prems(3) by force
-    show "wf_stmt \<Gamma> F \<Delta> (Cwhile b I C)"
+    show "wf_stmt \<Gamma> F (Cwhile b I C)"
       using Cwhile.prems(1) by auto
-    fix P Q show "invariant_translate \<Gamma> F \<Delta> P C Q"
+    fix P Q show "invariant_translate \<Gamma> P C Q"
     proof (rule Cwhile(1)[of P Q])
-      show "wf_stmt \<Gamma> F \<Delta> C"
+      show "wf_stmt \<Gamma> F C"
         using Cwhile.prems(1) by auto
-      show "well_typed_cmd \<Delta> C"
+      show "well_typed_cmd tcfe C"
         using Cwhile.prems(2) by auto
-      have "ConcreteSemantics.wf_abs_stmt \<Delta> (Inhale (?I \<inter> assertify_bexp b);; fst (translate \<Gamma> F C);; Exhale ?I)"
+      have "ConcreteSemantics.wf_abs_stmt tcfe (Inhale (?I \<inter> assertify_bexp b);; fst (translate \<Gamma> C);; Exhale ?I)"
         using Cwhile.prems(4) by fastforce
-      then show "ConcreteSemantics.wf_abs_stmt \<Delta> (fst (translate \<Gamma> F C))" by force
-      show "\<And>Cv. Cv \<in> snd (translate \<Gamma> F C) \<Longrightarrow> ConcreteSemantics.wf_abs_stmt \<Delta> Cv"
+      then show "ConcreteSemantics.wf_abs_stmt tcfe (fst (translate \<Gamma> C))" by force
+      show "\<And>Cv. Cv \<in> snd (translate \<Gamma> C) \<Longrightarrow> ConcreteSemantics.wf_abs_stmt tcfe Cv"
         using Cwhile.prems(4) by auto
     qed (simp add: Cwhile)
   qed (simp add: Cwhile)
@@ -1042,45 +1076,45 @@ qed (simp_all add: invariant_translate_skip invariant_translate_free invariant_t
 
 
 theorem sound_translation:
-  assumes "wf_stmt \<Gamma> F \<Delta> C"
-      and "well_typed_cmd \<Delta> C"
-      and "ConcreteSemantics.wf_abs_stmt \<Delta> (fst (translate \<Gamma> F C))"
-      and "\<And>Cv. Cv \<in> snd (translate \<Gamma> F C) \<Longrightarrow> ConcreteSemantics.wf_abs_stmt \<Delta> Cv"
-      and "TypedEqui.wf_assertion \<Delta> P \<and> TypedEqui.wf_assertion \<Delta> Q"
-      and "ConcreteSemantics.self_framing_and_typed \<Delta> P \<and> TypedEqui.typed_assertion \<Delta> P"
+  assumes "wf_stmt \<Gamma> F C"
+      and "well_typed_cmd tcfe C"
+      and "ConcreteSemantics.wf_abs_stmt tcfe (fst (translate \<Gamma> C))"
+      and "\<And>Cv. Cv \<in> snd (translate \<Gamma> C) \<Longrightarrow> ConcreteSemantics.wf_abs_stmt tcfe Cv"
+      and "TypedEqui.wf_assertion tcfe P \<and> TypedEqui.wf_assertion tcfe Q"
+      and "ConcreteSemantics.self_framing_and_typed tcfe P \<and> TypedEqui.typed_assertion tcfe P"
 
-      and "ConcreteSemantics.verifies_set \<Delta> (atrue \<Delta>) (Inhale P;; fst (translate \<Gamma> F C);; Exhale Q)"
-      and "\<And>Cv. Cv \<in> snd (translate \<Gamma> F C) \<Longrightarrow> ConcreteSemantics.verifies_set \<Delta> (atrue \<Delta>) Cv"
+      and "ConcreteSemantics.verifies_set tcfe (atrue tcfe) (Inhale P;; fst (translate \<Gamma> C);; Exhale Q)"
+      and "\<And>Cv. Cv \<in> snd (translate \<Gamma> C) \<Longrightarrow> ConcreteSemantics.verifies_set tcfe (atrue tcfe) Cv"
 
-      and "TypedEqui.wf_context \<Delta>"
-    shows "\<Delta> \<turnstile>CSL [P \<otimes> atrue \<Delta>] C [Q \<otimes> atrue \<Delta>]"
+      and "TypedEqui.wf_context tcfe"
+    shows "tcfe \<turnstile>CSL [P \<otimes> atrue tcfe] C [Q \<otimes> atrue tcfe]"
 proof -
-  obtain B where "ConcreteSemantics.SL_proof \<Delta> (atrue \<Delta>) (Inhale P;; fst (translate \<Gamma> F C);; Exhale Q) B"
+  obtain B where "ConcreteSemantics.SL_proof tcfe (atrue tcfe) (Inhale P;; fst (translate \<Gamma> C);; Exhale Q) B"
     by (metis ConcreteSemantics.Viper_implies_SL_proof ConcreteSemantics.wf_abs_stmt.simps(2) ConcreteSemantics.wf_abs_stmt.simps(3) ConcreteSemantics.wf_abs_stmt.simps(7) assms(3) assms(5) assms(7) atrue_self_framing_and_typed(1) atrue_self_framing_and_typed(2))
-  then obtain B' where "ConcreteSemantics.SL_proof \<Delta> (atrue \<Delta> \<otimes> P) (fst (translate \<Gamma> F C)) B'" "entails B' (B \<otimes> Q)"
+  then obtain B' where "ConcreteSemantics.SL_proof tcfe (atrue tcfe \<otimes> P) (fst (translate \<Gamma> C)) B'" "entails B' (B \<otimes> Q)"
     by blast
 
 
-  show "\<Delta> \<turnstile>CSL [P \<otimes> atrue \<Delta>] C [Q \<otimes> atrue \<Delta>]"
+  show "tcfe \<turnstile>CSL [P \<otimes> atrue tcfe] C [Q \<otimes> atrue tcfe]"
   proof (rule RuleCons)
-    show "\<Delta> \<turnstile>CSL [P \<otimes> atrue \<Delta> \<otimes> atrue \<Delta>] C [B' \<otimes> atrue \<Delta>]"
-    proof (rule invariant_translateE[of _ _ \<Delta> "P \<otimes> atrue \<Delta>" C])
-      show "ConcreteSemantics.SL_proof \<Delta> (P \<otimes> atrue \<Delta>) (fst (translate \<Gamma> F C)) B'"
-        by (metis \<open>ConcreteSemantics.SL_proof \<Delta> (atrue \<Delta> \<otimes> P) (fst (translate \<Gamma> F C)) B'\<close> add_set_commm)
-      show "invariant_translate \<Gamma> F \<Delta> (P \<otimes> atrue \<Delta>) C B'"
-        by (simp add: assms(1) assms(2) assms(3) assms(4) assms(9) invariant_translate_induct)
-      show "proof_obligations_valid \<Delta> (snd (translate \<Gamma> F C))"
+    show "tcfe \<turnstile>CSL [P \<otimes> atrue tcfe \<otimes> atrue tcfe] C [B' \<otimes> atrue tcfe]"
+    proof (rule invariant_translateE[of _ "P \<otimes> atrue tcfe" C])
+      show "ConcreteSemantics.SL_proof tcfe (P \<otimes> atrue tcfe) (fst (translate \<Gamma> C)) B'"
+        by (metis \<open>ConcreteSemantics.SL_proof tcfe (atrue tcfe \<otimes> P) (fst (translate \<Gamma> C)) B'\<close> add_set_commm)
+      show "invariant_translate \<Gamma> (P \<otimes> atrue tcfe) C B'"
+        by (meson assms(1) assms(2) assms(3) assms(4) invariant_translate_induct wf_context_type_context)
+      show "proof_obligations_valid (snd (translate \<Gamma> C))"
         unfolding proof_obligations_valid_def
       proof clarify
-        fix Cv assume "Cv \<in> snd (translate \<Gamma> F C)"
-        then show "\<exists>B. ConcreteSemantics.SL_proof \<Delta> (atrue \<Delta>) Cv B"
+        fix Cv assume "Cv \<in> snd (translate \<Gamma> C)"
+        then show "\<exists>B. ConcreteSemantics.SL_proof tcfe (atrue tcfe) Cv B"
           by (simp add: ConcreteSemantics.Viper_implies_SL_proof assms(4) assms(8))
       qed
     qed
-    show "P \<otimes> atrue \<Delta> \<subseteq> P \<otimes> atrue \<Delta> \<otimes> atrue \<Delta>"
+    show "P \<otimes> atrue tcfe \<subseteq> P \<otimes> atrue tcfe \<otimes> atrue tcfe"
       by (simp add: add_set_asso atrue_twice_equal)
-    show "B' \<otimes> atrue \<Delta> \<subseteq> Q \<otimes> atrue \<Delta>"
-      by (smt (verit, ccfv_SIG) ConcreteSemantics.proofs_are_self_framing_and_typed ConcreteSemantics.semantics_axioms \<open>ConcreteSemantics.SL_proof \<Delta> (atrue \<Delta>) (abs_stmt.Inhale P ;; fst (translate \<Gamma> F C) ;; abs_stmt.Exhale Q) B\<close> \<open>entails B' (B \<otimes> Q)\<close> add_set_mono assms(3) assms(5) atrue_twice_equal drop_conjunct_entails entails_def order.trans semantics.wf_abs_stmt.simps(2) semantics.wf_abs_stmt.simps(3) semantics.wf_abs_stmt.simps(7))
+    show "B' \<otimes> atrue tcfe \<subseteq> Q \<otimes> atrue tcfe"
+      by (smt (verit, ccfv_SIG) ConcreteSemantics.proofs_are_self_framing_and_typed ConcreteSemantics.semantics_axioms \<open>ConcreteSemantics.SL_proof tcfe (atrue tcfe) (abs_stmt.Inhale P ;; fst (translate \<Gamma> C) ;; abs_stmt.Exhale Q) B\<close> \<open>entails B' (B \<otimes> Q)\<close> add_set_mono assms(3) assms(5) atrue_twice_equal drop_conjunct_entails entails_def order.trans semantics.wf_abs_stmt.simps(2) semantics.wf_abs_stmt.simps(3) semantics.wf_abs_stmt.simps(7))
   qed
 qed
 
