simple-frontend/SyntacticTranslation.thy
@@ -6,30 +6,43 @@ fun translate_binop :: "int_binop \<Rightarrow> binop" where
   "translate_binop Add = binop.Add"
 | "translate_binop Sub = binop.Sub"
 | "translate_binop Mult = binop.Mult"
-| "translate_binop Mod = binop.Mod"
 
 fun translate_exp where
   "translate_exp (Evar x) = Var x"
 | "translate_exp (Elit l) = ELit (LInt l)"
 | "translate_exp (Ebinop e1 op e2) = Binop (translate_exp e1) (translate_binop op) (translate_exp e2)"
 
-term binop.Add
-
 fun translate_bexp where
   "translate_bexp (Beq e1 e2) = Binop (translate_exp e1) Eq (translate_exp e2)"
 | "translate_bexp (Band e1 e2) = Binop (translate_bexp e1) And (translate_bexp e2)"
 | "translate_bexp (Bnot e) = Unop Not (translate_bexp e)"
 
+(*
+record ('v, 'a) interp =
+  domains :: "'v \<Rightarrow> abs_type"
+  predicates :: "'v predicate_loc \<rightharpoonup> 'a set"
+  funs :: "function_ident \<Rightarrow> 'v val list \<Rightarrow> 'a \<rightharpoonup> 'v val"
+
+record ('v, 'c) abs_type_context =
+  variables :: "var \<rightharpoonup> 'v abs_vtyp"
+  custom_context :: 'c
+*)
+(*
+custom_context \<Delta> = type_ctxt_heap
+*)
 lemma translation_correct_exp:
-  "make_semantic_exp \<Delta> (translate_exp e) = semantify_exp e"
+  assumes "TypedEqui.typed type_ctxt_front_end \<omega>"
+(* Also needs something about typed program! *)
+  shows "make_semantic_exp \<Delta> (translate_exp e) \<omega> = semantify_exp e \<omega>"
   unfolding make_semantic_exp_def semantify_exp_def
 proof (induct e)
   case (Evar x)
+(* One can be none, the other one not... *)
   then show ?case sorry
 next
   case (Elit x)
-(* One can be none, the other one not... *)
-  show ?case
+  show ?case sorry
+(*
   proof (rule ext)
     fix \<omega>
     have "(if \<exists>v. \<Delta> \<turnstile> \<langle>translate_exp (Elit x);\<omega>\<rangle> [\<Down>] Val v then Some (SOME v. \<Delta> \<turnstile> \<langle>translate_exp (Elit x);\<omega>\<rangle> [\<Down>] Val v) else None)
@@ -49,14 +62,27 @@ next
          Some (VInt (edenot (Elit x) (get_store \<omega>)))"
       by fastforce
   qed
+*)
 next
   case (Ebinop e1 bop e2)
   then show ?case sorry
 qed
 
 lemma translation_correct_bexp:
-  "make_semantic_bexp \<Delta> (translate_bexp e) = semantify_bexp e"
-  sorry
+  assumes "TypedEqui.typed type_ctxt_front_end \<omega>"
+(* Also needs something about typed program! *)
+  shows "make_semantic_bexp \<Delta> (translate_bexp e) \<omega> = semantify_bexp e \<omega>"
+  unfolding make_semantic_bexp_def semantify_bexp_def
+proof (induct e)
+  case (Beq e1 e2)
+  then show ?case sorry
+next
+  case (Band e1 e2)
+  then show ?case sorry
+next
+  case (Bnot e)
+  then show ?case sorry
+qed
 
 definition syntactic_translate_addr :: "var \<Rightarrow> pure_exp" where
   "syntactic_translate_addr r = Var r"
@@ -73,9 +99,9 @@ proof (rule ext)
 qed
 
 lemma sound_translate_heap_loc:
-  "make_semantic_exp \<Delta> (syntactic_translate_heap_loc r) = semantify_heap_loc r"
+  "make_semantic_exp \<Gamma> (syntactic_translate_heap_loc r) = semantify_heap_loc r"
 proof (rule ext)
-  fix \<omega> show "make_semantic_exp \<Delta> (syntactic_translate_heap_loc r) \<omega> = semantify_heap_loc r \<omega>"
+  fix \<omega> show "make_semantic_exp \<Gamma> (syntactic_translate_heap_loc r) \<omega> = semantify_heap_loc r \<omega>"
     unfolding make_semantic_exp_def syntactic_translate_heap_loc_def semantify_heap_loc_def
     by (smt (verit) RedAccField2Val_case RedVar RedVar2Val_case get_address_simp option.sel red_pure_simps(6) someI_ex)
 qed
@@ -89,55 +115,104 @@ lemma make_semantic_inter_1:
   sorry
 
 lemma make_semantic_inter_2:
-  "make_semantic_assertion \<Delta> F (I && Atomic (Pure (translate_bexp b))) = (make_semantic_assertion \<Delta> F I) \<inter> assertify_bexp b"
+  "make_semantic_assertion \<Delta> type_ctxt_front_end_syntactic (I && Atomic (Pure (translate_bexp b))) = (make_semantic_assertion \<Delta> type_ctxt_front_end_syntactic I) \<inter> assertify_bexp b"
 proof
-  show "make_semantic_assertion \<Delta> F (I && Atomic (Pure (translate_bexp b))) \<subseteq> make_semantic_assertion \<Delta> F I \<inter> assertify_bexp b"
+  show "make_semantic_assertion \<Delta> type_ctxt_front_end_syntactic (I && Atomic (Pure (translate_bexp b))) \<subseteq> make_semantic_assertion \<Delta> type_ctxt_front_end_syntactic I \<inter> assertify_bexp b"
     unfolding make_semantic_assertion_def well_typedly_def
   proof
-    fix \<omega> assume "\<omega> \<in> \<langle>\<Delta>, F\<rangle> \<Turnstile> \<langle>I && Atomic (Pure (translate_bexp b))\<rangle> \<inter> {\<omega> |\<omega>. well_typed (map_option (make_semantic_vtyp \<Delta>) \<circ> F) (get_abs_state \<omega>)}"
-    then obtain i p where ip: "Some \<omega> = i \<oplus> p" "i \<in> \<langle>\<Delta>, F\<rangle> \<Turnstile> \<langle>I\<rangle>" "p \<in> \<langle>\<Delta>, F\<rangle> \<Turnstile> \<langle>Atomic (Pure (translate_bexp b))\<rangle>"
-      by (smt (verit, ccfv_SIG) IntD1 sat_set.simps(4) x_elem_set_product)
-    then have "\<omega> \<in> \<langle>\<Delta>, F\<rangle> \<Turnstile> \<langle>I\<rangle>" (* up_closed, p is pure *)
-      sorry
+    fix \<omega> assume "\<omega> \<in> Set.filter (typed (make_context_semantic \<Delta> type_ctxt_front_end_syntactic)) (\<langle>\<Delta>, snd type_ctxt_front_end_syntactic\<rangle> \<Turnstile> \<langle>I && Atomic (Pure (translate_bexp b))\<rangle>)"
+    then obtain i p where ip: "Some \<omega> = i \<oplus> p" "i \<in> \<langle>\<Delta>, snd type_ctxt_front_end_syntactic\<rangle> \<Turnstile> \<langle>I\<rangle>" "p \<in> \<langle>\<Delta>, snd type_ctxt_front_end_syntactic\<rangle> \<Turnstile> \<langle>Atomic (Pure (translate_bexp b))\<rangle>"     
+      by (smt (verit, ccfv_threshold) member_filter sat_set.simps(4) snd_conv type_ctxt_front_end_syntactic_def x_elem_set_product)
+    then have "pure p"
+      by (metis CollectD Instantiation.atomic_assert.simps(1) Int_iff corely_def emp_core_def red_pure_assert_def sat_set.simps(1))
+    then have "\<omega> \<in> \<langle>\<Delta>, snd type_ctxt_front_end_syntactic\<rangle> \<Turnstile> \<langle>I\<rangle>"
+      using ip(1-2)
+      sorry (* TODO: Prove *)
     moreover have "get_store \<omega> = get_store p"
       by (metis \<open>Some \<omega> = i \<oplus> p\<close> commutative full_add_charact(1))
-    moreover have "bdenot b (get_store p)"
-      using translation_correct_bexp[of \<Delta> b] ip(3)
+    moreover have "typed type_ctxt_front_end \<omega>" using make_context_semantic_type_ctxt
+      by (metis \<open>\<omega> \<in> Set.filter (typed (make_context_semantic \<Delta> type_ctxt_front_end_syntactic)) (\<langle>\<Delta>, snd type_ctxt_front_end_syntactic\<rangle> \<Turnstile> \<langle>I && Atomic (Pure (translate_bexp b))\<rangle>)\<close> member_filter)
+    then have "TypedEqui.typed type_ctxt_front_end p"
+      by (metis TypedEqui.typed_smaller commutative greater_def ip(1))
+    then have "bdenot b (get_store p)"
+      using translation_correct_bexp[of p _ b] ip(3)
       unfolding semantify_bexp_def make_semantic_bexp_def assertify_bexp_def sat_set.simps atomic_assert.simps red_pure_assert_def
         corely_def
-      by (metis (no_types, lifting) CollectD IntD1 option.inject)
-
+      by (metis Int_Collect inf.commute option.inject)
     ultimately have "\<omega> \<in> assertify_bexp b"
-      using translation_correct_bexp[of \<Delta> b] ip(3) unfolding semantify_bexp_def make_semantic_bexp_def assertify_bexp_def
+      using translation_correct_bexp[of _ _ b] ip(3) unfolding semantify_bexp_def make_semantic_bexp_def assertify_bexp_def
       by simp
-    then show "\<omega> \<in> \<langle>\<Delta>, F\<rangle> \<Turnstile> \<langle>I\<rangle> \<inter> {\<omega> |\<omega>. well_typed (map_option (make_semantic_vtyp \<Delta>) \<circ> F) (get_abs_state \<omega>)} \<inter> assertify_bexp b"
-      using \<open>\<omega> \<in> \<langle>\<Delta>, F\<rangle> \<Turnstile> \<langle>I && Atomic (Pure (translate_bexp b))\<rangle> \<inter> {\<omega> |\<omega>. well_typed (map_option (make_semantic_vtyp \<Delta>) \<circ> F) (get_abs_state \<omega>)}\<close>
-      using \<open>\<omega> \<in> \<langle>\<Delta>, F\<rangle> \<Turnstile> \<langle>I\<rangle>\<close> by blast
+    then show "\<omega> \<in> Set.filter (typed (make_context_semantic \<Delta> type_ctxt_front_end_syntactic)) (\<langle>\<Delta>, snd type_ctxt_front_end_syntactic\<rangle> \<Turnstile> \<langle>I\<rangle>) \<inter> assertify_bexp b"
+      by (simp add: \<open>\<omega> \<in> \<langle>\<Delta>, snd type_ctxt_front_end_syntactic\<rangle> \<Turnstile> \<langle>I\<rangle>\<close> \<open>typed type_ctxt_front_end \<omega>\<close> make_context_semantic_type_ctxt)
   qed
-  show "make_semantic_assertion \<Delta> F I \<inter> assertify_bexp b \<subseteq> make_semantic_assertion \<Delta> F (I && Atomic (Pure (translate_bexp b)))"
+  show "make_semantic_assertion \<Delta> type_ctxt_front_end_syntactic I \<inter> assertify_bexp b
+    \<subseteq> make_semantic_assertion \<Delta> type_ctxt_front_end_syntactic (I && Atomic (Pure (translate_bexp b)))"
     unfolding make_semantic_assertion_def assertify_bexp_def well_typedly_def
   proof
     fix \<omega>
-    assume asm0: "\<omega> \<in> \<langle>\<Delta>, F\<rangle> \<Turnstile> \<langle>I\<rangle> \<inter> {\<omega> |\<omega>. well_typed (map_option (make_semantic_vtyp \<Delta>) \<circ> F) (get_abs_state \<omega>)} \<inter> {\<omega> |\<omega>. bdenot b (get_store \<omega>)}"
+    assume asm0: "\<omega> \<in> Set.filter (typed (make_context_semantic \<Delta> type_ctxt_front_end_syntactic)) (\<langle>\<Delta>, snd type_ctxt_front_end_syntactic\<rangle> \<Turnstile> \<langle>I\<rangle>) \<inter>
+             {\<omega> |\<omega>. bdenot b (get_store \<omega>)}"
     moreover have "Some \<omega> = \<omega> \<oplus> |\<omega>|"
       using core_is_smaller by auto
-    moreover have "|\<omega>| \<in> \<langle>\<Delta>, F\<rangle> \<Turnstile> \<langle>Atomic (Pure (translate_bexp b))\<rangle>"
-      using translation_correct_bexp[of \<Delta> b] asm0
+    moreover have "TypedEqui.typed type_ctxt_front_end \<omega>"
+      by (metis IntD1 asm0 make_context_semantic_type_ctxt member_filter)
+    then have "|\<omega>| \<in> \<langle>\<Delta>, snd type_ctxt_front_end_syntactic\<rangle> \<Turnstile> \<langle>Atomic (Pure (translate_bexp b))\<rangle>"
+      using translation_correct_bexp[of _ _ b] asm0
       unfolding sat_set.simps atomic_assert.simps red_pure_assert_def corely_def semantify_bexp_def make_semantic_bexp_def
-      by (metis (no_types, lifting) Int_Collect Int_iff core_charact(1) core_in_emp_core option.distinct(1) option.inject)
-    ultimately show "\<omega> \<in> \<langle>\<Delta>, F\<rangle> \<Turnstile> \<langle>I && Atomic (Pure (translate_bexp b))\<rangle> \<inter> {\<omega> |\<omega>. well_typed (map_option (make_semantic_vtyp \<Delta>) \<circ> F) (get_abs_state \<omega>)}"
-      using x_elem_set_product by fastforce
+      by (metis (no_types, lifting) Int_iff TypedEqui.typed_core core_charact(1) core_in_emp_core mem_Collect_eq option.distinct(1) option.inject)
+    ultimately show "\<omega> \<in> Set.filter (typed (make_context_semantic \<Delta> type_ctxt_front_end_syntactic))
+               (\<langle>\<Delta>, snd type_ctxt_front_end_syntactic\<rangle> \<Turnstile> \<langle>I && Atomic (Pure (translate_bexp b))\<rangle>)"
+      using x_elem_set_product
+      by (smt (verit, ccfv_threshold) IntD1 member_filter sat_set.simps(4) snd_conv type_ctxt_front_end_syntactic_def)
   qed
 qed
 
 
 lemma full_ownership_translation_sound:
-  "make_semantic_assertion \<Delta> F (Atomic (Acc (Var r) field_val (PureExp (ELit (LPerm 1))))) = Stabilize (full_ownership r)"
-  sorry
+  "make_semantic_assertion \<Delta> type_ctxt_front_end_syntactic (Atomic (Acc (Var r) field_val (PureExp (ELit (LPerm 1))))) = typed_stabilize (full_ownership r)"
+  unfolding make_semantic_assertion_def well_typedly_def full_ownership_def sat_set.simps atomic_assert.simps
+    TypedEqui.Stabilize_typed_def red_pure_assert_def corely_def emp_core_def
+  apply simp
+proof -
+  have "(\<Union>x xa xb.
+         \<Delta> \<turnstile> \<langle>Var r\<rangle> [\<Down>] Val (VRef x) \<otimes> \<llangle>snd type_ctxt_front_end_syntactic field_val = Some xb\<rrangle> \<otimes>
+         (\<Union>p'. \<Delta> \<turnstile> \<langle>ELit WritePerm\<rangle> [\<Down>] Val (VPerm p') \<otimes> \<llangle>xa = Some p'\<rrangle>) \<otimes>
+         acc \<Delta> xb x field_val xa) =
+ (Stabilize {\<omega>. \<exists>l. get_store \<omega> r = Some (VRef (Address l)) \<and> get_m \<omega> (l, field_val) = 1})" (is "?A = ?B")
+  proof
+    show "?A \<subseteq> ?B"
+    proof
+      fix \<omega> assume asm0: "\<omega> \<in> ?A"
+      then obtain x xa xb where "\<omega> \<in> \<Delta> \<turnstile> \<langle>Var r\<rangle> [\<Down>] Val (VRef x) \<otimes> \<llangle>snd type_ctxt_front_end_syntactic field_val = Some xb\<rrangle> \<otimes>
+           (\<Union>p'. \<Delta> \<turnstile> \<langle>ELit WritePerm\<rangle> [\<Down>] Val (VPerm p') \<otimes> \<llangle>xa = Some p'\<rrangle>) \<otimes>
+           acc \<Delta> xb x field_val xa"
+        by (smt (z3) UN_iff snd_conv type_ctxt_front_end_syntactic_def)
+      then show "\<omega> \<in> ?B"
+        sorry
+    qed
+    show "?B \<subseteq> ?A"
+    proof
+      fix \<omega> assume asm0: "\<omega> \<in> ?B"
+      then obtain l where "get_store (stabilize \<omega>) r = Some (VRef (Address l))" "get_m (stabilize \<omega>) (l, field_val) = 1"
+        by auto
+
+      then show "\<omega> \<in> ?A" sorry
+    qed
+  qed
+  then show "Set.filter (typed tcfe)
+     (\<Union>x xa xb.
+         {\<omega>. \<Delta> \<turnstile> \<langle>Var r;\<omega>\<rangle> [\<Down>] Val (VRef x)} \<inter> Collect pure \<otimes> \<llangle>snd type_ctxt_front_end_syntactic field_val = Some xb\<rrangle> \<otimes>
+         (\<Union>p'. {\<omega>. \<Delta> \<turnstile> \<langle>ELit WritePerm;\<omega>\<rangle> [\<Down>] Val (VPerm p')} \<inter> Collect pure \<otimes> \<llangle>xa = Some p'\<rrangle>) \<otimes>
+         acc \<Delta> xb x field_val xa) =
+    Set.filter (typed tcfe) (Stabilize {\<omega>. \<exists>l. get_store \<omega> r = Some (VRef (Address l)) \<and> get_m \<omega> (l, field_val) = 1})"
+    unfolding red_pure_assert_def corely_def emp_core_def
+    by fastforce
+qed
+
 
 lemma full_ownership_with_val_sound:
   "make_semantic_assertion \<Delta> F (Atomic (Acc (Var r) field_val (PureExp (ELit (LPerm 1)))) && Atomic (Pure (FieldAcc (Var r) field_val)))
-  = full_ownership_with_val r e"
+  = typed_stabilize (full_ownership_with_val r e)"
   sorry
 
 
@@ -179,9 +254,48 @@ lemma havoc_list_n_havoc_same:
   "compile \<Delta> F (n_havoc l) = ConcreteSemantics.havoc_list l"
   by (induct l) simp_all
 
+thm ConcreteSemantics.verifies_set_def ConcreteSemantics.verifies_def
+
+lemma translation_refines:
+  assumes "ConcreteSemantics.red_stmt tcfe (compile \<Delta> F (fst (translate_syn \<Delta> F C))) \<omega> S"
+      and "typed tcfe \<omega>"
+      and "stable \<omega>"
+  shows "ConcreteSemantics.red_stmt tcfe (fst (translate \<Delta> C)) \<omega> S"
+  using assms
+proof (induct C arbitrary: \<omega> S)
+  case (Cassign x1 x2)
+  then show ?case sorry
+next
+  case (Cwrite x1 x2)
+  then show ?case sorry
+next
+  case (Calloc x1 x2)
+  then show ?case sorry
+next
+  case (Cfree x)
+  then show ?case sorry
+next
+  case (Cseq C1 C2)
+  then show ?case sorry
+next
+  case (Cpar x1 C1 x3 x4 C2 x6a)
+  then show ?case sorry
+next
+  case (Cif x1 C1 C2)
+  then show ?case sorry
+next
+  case (Cwhile x1 x2 C)
+  then show ?case sorry
+qed (simp_all add: sound_translate_heap_loc)
+
+(*
+      and "ConcreteSemantics.verifies_set tcfe (atrue tcfe) (Inhale P;; fst (translate \<Gamma> C);; Exhale Q)"
+      and "\<And>Cv. Cv \<in> snd (translate \<Gamma> C) \<Longrightarrow> ConcreteSemantics.verifies_set tcfe (atrue tcfe) Cv"
+*)
+
 (* main theorem *)
 lemma translation_same:
-  "compile \<Delta> F (fst (translate_syn \<Delta> F C)) = fst (translate \<Delta> F C) \<and> compile \<Delta> F ` (snd (translate_syn \<Delta> F C)) = snd (translate \<Delta> F C)"
+  "compile \<Delta> F (fst (translate_syn \<Delta> F C)) = fst (translate \<Delta> C) \<and> compile \<Delta> F ` (snd (translate_syn \<Delta> F C)) = snd (translate \<Delta> C)"
 proof (induct C)
   case (Cassign x1 x2)
   then show ?case using translation_correct_exp compile.simps(5) translate.simps(2) translate_syn.simps(2)
